Lots of blind progress on proofs, but I screwed up R_env
I have to drop one argument of R_env right now, for the proofs to make sense.

ecoop17/dsubsup_total_rec_monotone_part2.v
@@ -157,1163 +157,1255 @@ Definition R_env venv genv tenv :=
        forall n, vtp genv [] TX n vx).
 
 
-(* (* automation *) *)
-(* Hint Unfold venv. *)
-(* Hint Unfold tenv. *)
+(* automation *)
+Hint Unfold venv.
+Hint Unfold tenv.
 
-(* Hint Unfold open. *)
-(* Hint Unfold indexr. *)
-(* Hint Unfold length. *)
+Hint Unfold open.
+Hint Unfold indexr.
+Hint Unfold length.
 
-(* (* Hint Unfold R. *) *)
-(* Hint Unfold R_env. *)
+(* Hint Unfold R. *)
+Hint Unfold R_env.
 
-(* Hint Constructors ty. *)
-(* Hint Constructors tm. *)
-(* Hint Constructors vl. *)
+Hint Constructors ty.
+Hint Constructors tm.
+Hint Constructors vl.
 
-(* Hint Constructors closed. *)
-(* Hint Constructors has_type. *)
-(* Hint Constructors stp. *)
+Hint Constructors closed.
+Hint Constructors has_type.
+Hint Constructors stp.
 
-(* Hint Constructors option. *)
-(* Hint Constructors list. *)
+Hint Constructors option.
+Hint Constructors list.
 
-(* Hint Resolve ex_intro. *)
+Hint Resolve ex_intro.
 
-(* (* ############################################################ *) *)
-(* (* Examples *) *)
-(* (* ############################################################ *) *)
+(* ############################################################ *)
+(* Examples *)
+(* ############################################################ *)
 
 
-(* Ltac crush := *)
-(*   try solve [eapply stp_selx; compute; eauto; crush]; *)
-(*   try solve [eapply stp_selax; compute; eauto; crush]; *)
-(*   try solve [econstructor; compute; eauto; crush]; *)
-(*   try solve [eapply t_sub; crush]. *)
+Ltac crush :=
+  try solve [eapply stp_selx; compute; eauto; crush];
+  try solve [eapply stp_selax; compute; eauto; crush];
+  try solve [econstructor; compute; eauto; crush];
+  try solve [eapply t_sub; crush].
 
-(* (* define polymorphic identity function *) *)
+(* define polymorphic identity function *)
 
-(* Definition polyId := TAll (TMem TBot TTop) (TAll (TSel (varB 0)) (TSel (varB 1))). *)
+Definition polyId := TAll (TMem TBot TTop) (TAll (TSel (varB 0)) (TSel (varB 1))).
 
-(* Example ex10: has_type [] (tabs (TMem TBot TTop) (tabs (TSel (varF 0)) (tvar 1))) polyId. *)
-(* Proof.  *)
-(*   crush. *)
-(* Qed. *)
+Example ex10: has_type [] (tabs (TMem TBot TTop) (tabs (TSel (varF 0)) (tvar 1))) polyId.
+Proof.
+  crush.
+Qed.
 
-(* (* *)
-(* (* instantiate it to TTop *) *)
+
+(* instantiate it to TTop *)
 (* Example ex20: has_type [polyId] (tapp (tvar 0) (ttyp TTop)) (TAll TTop TTop). *)
-(* Proof.  *)
+(* Proof. *)
 (*   crush. *)
 (* Qed. *)
-(* *) *)
-
-(* (* ############################################################ *) *)
-(* (* Proofs *) *)
-(* (* ############################################################ *) *)
-
-
-
-(* (* ## Extension, Regularity ## *) *)
-
-(* Lemma wf_length : forall vs gs ts, *)
-(*                     R_env vs gs ts -> *)
-(*                     (length vs = length ts). *)
-(* Proof. *)
-(*   intros. induction H. auto. *)
-(* Qed. *)
-
-(* Lemma wf_length2 : forall vs gs ts, *)
-(*                     R_env vs gs ts -> *)
-(*                     (length gs = length ts). *)
-(* Proof. *)
-(*   intros. destruct H. destruct H0. auto. *)
-(* Qed. *)
-
-
-(* Hint Immediate wf_length. *)
-
-(* Lemma indexr_max : forall X vs n (T: X), *)
-(*                        indexr n vs = Some T -> *)
-(*                        n < length vs. *)
-(* Proof. *)
-(*   intros X vs. induction vs. *)
-(*   - Case "nil". intros. inversion H. *)
-(*   - Case "cons". *)
-(*     intros. inversion H. *)
-(*     case_eq (beq_nat n (length vs)); intros E2. *)
-(*     + SSCase "hit". *)
-(*       eapply beq_nat_true in E2. subst n. compute. eauto. *)
-(*     + SSCase "miss". *)
-(*       rewrite E2 in H1. *)
-(*       assert (n < length vs). eapply IHvs. apply H1. *)
-(*       compute. eauto. *)
-(* Qed. *)
-
-(* Lemma le_xx : forall a b, *)
-(*                        a <= b -> *)
-(*                        exists E, le_lt_dec a b = left E. *)
-(* Proof. intros. *)
-(*   case_eq (le_lt_dec a b). intros. eauto. *)
-(*   intros. omega. *)
-(* Qed. *)
-(* Lemma le_yy : forall a b, *)
-(*                        a > b -> *)
-(*                        exists E, le_lt_dec a b = right E. *)
-(* Proof. intros. *)
-(*   case_eq (le_lt_dec a b). intros. omega. *)
-(*   intros. eauto. *)
-(* Qed. *)
-
-(* Lemma indexr_extend : forall X vs n x (T: X), *)
-(*                        indexr n vs = Some T -> *)
-(*                        indexr n (x::vs) = Some T. *)
-
-(* Proof. *)
-(*   intros. *)
-(*   assert (n < length vs). eapply indexr_max. eauto. *)
-(*   assert (beq_nat n (length vs) = false) as E. eapply beq_nat_false_iff. omega. *)
-(*   unfold indexr. unfold indexr in H. rewrite H. rewrite E. reflexivity. *)
-(* Qed. *)
-
-(* (* splicing -- for stp_extend. *) *)
-
-(* Fixpoint splice n (T : ty) {struct T} : ty := *)
-(*   match T with *)
-(*     | TTop         => TTop *)
-(*     | TBot         => TBot *)
-(*     | TAll T1 T2   => TAll (splice n T1) (splice n T2) *)
-(*     | TSel (varF i) => TSel (varF i) *)
-(*     | TSel (varB i) => TSel (varB i) *)
-(*     | TSel (varH i) => if le_lt_dec n i then TSel (varH (i+1)) else TSel (varH i) *)
-(*     | TMem T1 T2   => TMem (splice n T1) (splice n T2) *)
-(*     | TBind T      => TBind (splice n T) *)
-(*     | TAnd T1 T2   => TAnd (splice n T1) (splice n T2) *)
-(*   end. *)
-
-(* Definition spliceat n (V: (venv*ty)) := *)
-(*   match V with *)
-(*     | (G,T) => (G,splice n T) *)
-(*   end. *)
-
-(* Lemma splice_open_permute: forall {X} (G0:list X) T2 n j, *)
-(* (open_rec j (varH (n + S (length G0))) (splice (length G0) T2)) = *)
-(* (splice (length G0) (open_rec j (varH (n + length G0)) T2)). *)
-(* Proof. *)
-(*   intros X G T. induction T; intros; simpl; eauto; *)
-(*   try rewrite IHT1; try rewrite IHT2; try rewrite IHT; eauto; *)
-(*   destruct v; eauto. *)
-
-(*   case_eq (le_lt_dec (length G) i); intros E LE; simpl; eauto. *)
-(*   rewrite LE. eauto. *)
-(*   rewrite LE. eauto. *)
-(*   case_eq (beq_nat j i); intros E; simpl; eauto. *)
-(*   case_eq (le_lt_dec (length G) (n + length G)); intros EL LE. *)
-(*   rewrite E. *)
-(*   assert (n + S (length G) = n + length G + 1). omega. *)
-(*   rewrite H. eauto. *)
-(*   omega. *)
-(*   rewrite E. eauto. *)
-(* Qed. *)
-
-(* Lemma indexr_splice_hi: forall G0 G2 x0 v1 T, *)
-(*     indexr x0 (G2 ++ G0) = Some T -> *)
-(*     length G0 <= x0 -> *)
-(*     indexr (x0 + 1) (map (splice (length G0)) G2 ++ v1 :: G0) = Some (splice (length G0) T). *)
-(* Proof. *)
-(*   intros G0 G2. induction G2; intros. *)
-(*   - eapply indexr_max in H. simpl in H. omega. *)
-(*   - simpl in H. *)
-(*     case_eq (beq_nat x0 (length (G2 ++ G0))); intros E. *)
-(*     + rewrite E in H. inversion H. subst. simpl. *)
-(*       rewrite app_length in E. *)
-(*       rewrite app_length. rewrite map_length. simpl. *)
-(*       assert (beq_nat (x0 + 1) (length G2 + S (length G0)) = true). { *)
-(*         eapply beq_nat_true_iff. eapply beq_nat_true_iff in E. omega. *)
-(*       } *)
-(*       rewrite H1. eauto. *)
-(*     + rewrite E in H.  eapply IHG2 in H. eapply indexr_extend. eapply H. eauto. *)
-(* Qed. *)
-
-(* Lemma indexr_spliceat_hi: forall G0 G2 x0 v1 G T, *)
-(*     indexr x0 (G2 ++ G0) = Some (G, T) -> *)
-(*     length G0 <= x0 -> *)
-(*     indexr (x0 + 1) (map (spliceat (length G0)) G2 ++ v1 :: G0) = *)
-(*     Some (G, splice (length G0) T). *)
-(* Proof. *)
-(*   intros G0 G2. induction G2; intros. *)
-(*   - eapply indexr_max in H. simpl in H. omega. *)
-(*   - simpl in H. destruct a. *)
-(*     case_eq (beq_nat x0 (length (G2 ++ G0))); intros E. *)
-(*     + rewrite E in H. inversion H. subst. simpl. *)
-(*       rewrite app_length in E. *)
-(*       rewrite app_length. rewrite map_length. simpl. *)
-(*       assert (beq_nat (x0 + 1) (length G2 + S (length G0)) = true). { *)
-(*         eapply beq_nat_true_iff. eapply beq_nat_true_iff in E. omega. *)
-(*       } *)
-(*       rewrite H1. eauto. *)
-(*     + rewrite E in H.  eapply IHG2 in H. eapply indexr_extend. eapply H. eauto. *)
-(* Qed. *)
-
-(* Lemma plus_lt_contra: forall a b, *)
-(*   a + b < b -> False. *)
-(* Proof. *)
-(*   intros a b H. induction a. *)
-(*   - simpl in H. apply lt_irrefl in H. assumption. *)
-(*   - simpl in H. apply IHa. omega. *)
-(* Qed. *)
-
-(* Lemma indexr_splice_lo0: forall {X} G0 G2 x0 (T:X), *)
-(*     indexr x0 (G2 ++ G0) = Some T -> *)
-(*     x0 < length G0 -> *)
-(*     indexr x0 G0 = Some T. *)
-(* Proof. *)
-(*   intros X G0 G2. induction G2; intros. *)
-(*   - simpl in H. apply H. *)
-(*   - simpl in H. *)
-(*     case_eq (beq_nat x0 (length (G2 ++ G0))); intros E. *)
-(*     + eapply beq_nat_true_iff in E. subst. *)
-(*       rewrite app_length in H0. apply plus_lt_contra in H0. inversion H0. *)
-(*     + rewrite E in H. apply IHG2. apply H. apply H0. *)
-(* Qed. *)
-
-(* Lemma indexr_extend_mult: forall {X} G0 G2 x0 (T:X), *)
-(*     indexr x0 G0 = Some T -> *)
-(*     indexr x0 (G2++G0) = Some T. *)
-(* Proof. *)
-(*   intros X G0 G2. induction G2; intros. *)
-(*   - simpl. assumption. *)
-(*   - simpl. *)
-(*     case_eq (beq_nat x0 (length (G2 ++ G0))); intros E. *)
-(*     + eapply beq_nat_true_iff in E. *)
-(*       apply indexr_max in H. subst. *)
-(*       rewrite app_length in H. apply plus_lt_contra in H. inversion H. *)
-(*     + apply IHG2. assumption. *)
-(* Qed. *)
-
-(* Lemma indexr_splice_lo: forall G0 G2 x0 v1 T f, *)
-(*     indexr x0 (G2 ++ G0) = Some T -> *)
-(*     x0 < length G0 -> *)
-(*     indexr x0 (map (splice f) G2 ++ v1 :: G0) = Some T. *)
-(* Proof. *)
-(*   intros. *)
-(*   assert (indexr x0 G0 = Some T). eapply indexr_splice_lo0; eauto. *)
-(*   eapply indexr_extend_mult. eapply indexr_extend. eauto. *)
-(* Qed. *)
-
-(* Lemma indexr_spliceat_lo: forall G0 G2 x0 v1 G T f, *)
-(*     indexr x0 (G2 ++ G0) = Some (G, T) -> *)
-(*     x0 < length G0 -> *)
-(*     indexr x0 (map (spliceat f) G2 ++ v1 :: G0) = Some (G, T). *)
-(* Proof. *)
-(*   intros. *)
-(*   assert (indexr x0 G0 = Some (G, T)). eapply indexr_splice_lo0; eauto. *)
-(*   eapply indexr_extend_mult. eapply indexr_extend. eauto. *)
-(* Qed. *)
-
-(* Lemma closed_splice: forall i j k T n, *)
-(*   closed i j k T -> *)
-(*   closed i (S j) k (splice n T). *)
-(* Proof. *)
-(*   intros. induction H; simpl; eauto. *)
-(*   case_eq (le_lt_dec n x); intros E LE. *)
-(*   apply cl_selh. omega. *)
-(*   apply cl_selh. omega. *)
-(* Qed. *)
-
-(* Lemma map_splice_length_inc: forall G0 G2 v1, *)
-(*    (length (map (splice (length G0)) G2 ++ v1 :: G0)) = (S (length (G2 ++ G0))). *)
-(* Proof. *)
-(*   intros. rewrite app_length. rewrite map_length. induction G2. *)
-(*   - simpl. reflexivity. *)
-(*   - simpl. eauto. *)
-(* Qed. *)
-
-(* Lemma map_spliceat_length_inc: forall G0 G2 v1, *)
-(*    (length (map (spliceat (length G0)) G2 ++ v1 :: G0)) = (S (length (G2 ++ G0))). *)
-(* Proof. *)
-(*   intros. rewrite app_length. rewrite map_length. induction G2. *)
-(*   - simpl. reflexivity. *)
-(*   - simpl. eauto. *)
-(* Qed. *)
-
-(* Lemma closed_inc_mult: forall i j k T, *)
-(*   closed i j k T -> *)
-(*   forall i' j' k', *)
-(*   i' >= i -> j' >= j -> k' >= k -> *)
-(*   closed i' j' k' T. *)
-(* Proof. *)
-(*   intros i j k T H. induction H; intros; eauto; try solve [constructor; omega]. *)
-(*   - apply cl_all. apply IHclosed1; omega. apply IHclosed2; omega. *)
-(*   - constructor. apply IHclosed; omega. *)
-(* Qed. *)
-
-(* Lemma closed_inc: forall i j k T, *)
-(*   closed i j k T -> *)
-(*   closed i (S j) k T. *)
-(* Proof. *)
-(*   intros. apply (closed_inc_mult i j k T H i (S j) k); omega. *)
-(* Qed. *)
-
-(* Lemma closed_splice_idem: forall i j k T n, *)
-(*                             closed i j k T -> *)
-(*                             n >= j -> *)
-(*                             splice n T = T. *)
-(* Proof. *)
-(*   intros. induction H; eauto. *)
-(*   - (* TAll *) simpl. *)
-(*     rewrite IHclosed1. rewrite IHclosed2. *)
-(*     reflexivity. *)
-(*     assumption. assumption. *)
-(*   - (* TVarH *) simpl. *)
-(*     case_eq (le_lt_dec n x); intros E LE. omega. reflexivity. *)
-(*   - (* TMem *) simpl. *)
-(*     rewrite IHclosed1. rewrite IHclosed2. *)
-(*     reflexivity. *)
-(*     assumption. assumption. *)
-(*   - simpl. rewrite IHclosed. reflexivity. assumption. *)
-(*   - simpl. rewrite IHclosed1. rewrite IHclosed2. reflexivity. assumption. assumption. *)
-(* Qed. *)
-
-(* Lemma stp_closed : forall G GH T1 T2, *)
-(*                      stp G GH T1 T2 -> *)
-(*                      closed 0 (length GH) (length G) T1 /\ closed 0 (length GH) (length G) T2. *)
-(* Proof. *)
-(*   intros. induction H; *)
-(*     try solve [repeat ev; split; try inv_mem; eauto using indexr_max]. *)
-(* Qed. *)
-
-(* Lemma stp_closed2 : forall G1 GH T1 T2, *)
-(*                        stp G1 GH T1 T2 -> *)
-(*                        closed 0 (length GH) (length G1) T2. *)
-(* Proof. *)
-(*   intros. apply (proj2 (stp_closed G1 GH T1 T2 H)). *)
-(* Qed. *)
-
-(* Lemma stp_closed1 : forall G1 GH T1 T2, *)
-(*                        stp G1 GH T1 T2 -> *)
-(*                        closed 0 (length GH) (length G1) T1. *)
-(* Proof. *)
-(*   intros. apply (proj1 (stp_closed G1 GH T1 T2 H)). *)
-(* Qed. *)
-
-
-(* Lemma closed_upgrade: forall i j k i' T, *)
-(*  closed i j k T -> *)
-(*  i' >= i -> *)
-(*  closed i' j k T. *)
-(* Proof. *)
-(*  intros. apply (closed_inc_mult i j k T H i' j k); omega. *)
-(* Qed. *)
-
-(* Lemma closed_upgrade_free: forall i j k j' T, *)
-(*  closed i j k T -> *)
-(*  j' >= j -> *)
-(*  closed i j' k T. *)
-(* Proof. *)
-(*  intros. apply (closed_inc_mult i j k T H i j' k); omega. *)
-(* Qed. *)
-
-(* Lemma closed_upgrade_freef: forall i j k k' T, *)
-(*  closed i j k T -> *)
-(*  k' >= k -> *)
-(*  closed i j k' T. *)
-(* Proof. *)
-(*  intros. apply (closed_inc_mult i j k T H i j k'); omega. *)
-(* Qed. *)
-
-(* Lemma closed_open: forall i j k V T, closed (i+1) j k T -> closed i j k (TSel V) -> *)
-(*   closed i j k (open_rec i V T). *)
-(* Proof. *)
-(*   intros. generalize dependent i. *)
-(*   induction T; intros; inversion H; *)
-(*   try econstructor; *)
-(*   try eapply IHT1; eauto; try eapply IHT2; eauto; try eapply IHT; eauto. *)
-(*   eapply closed_upgrade. eauto. eauto. *)
-(*   - Case "TVarB". simpl. *)
-(*     case_eq (beq_nat i x); intros E. eauto. *)
-(*     econstructor. eapply beq_nat_false_iff in E. omega. *)
-(*   - eapply closed_upgrade. eassumption. omega. *)
-(* Qed. *)
-
-(* Lemma indexr_has: forall X (G: list X) x, *)
-(*   length G > x -> *)
-(*   exists v, indexr x G = Some v. *)
-(* Proof. *)
-(*   intros. remember (length G) as n. *)
-(*   generalize dependent x. *)
-(*   generalize dependent G. *)
-(*   induction n; intros; try omega. *)
-(*   destruct G; simpl. *)
-(*   - simpl in Heqn. inversion Heqn. *)
-(*   - simpl in Heqn. inversion Heqn. subst. *)
-(*     case_eq (beq_nat x (length G)); intros E. *)
-(*     + eexists. reflexivity. *)
-(*     + apply beq_nat_false in E. apply IHn; eauto. *)
-(*       omega. *)
-(* Qed. *)
-
-(* Lemma stp_refl_aux: forall n T G GH, *)
-(*   closed 0 (length GH) (length G) T -> *)
-(*   tsize_flat T < n -> *)
-(*   stp G GH T T. *)
-(* Proof. *)
-(*   intros n. induction n; intros; try omega. *)
-(*   inversion H; subst; eauto; *)
-(*   try solve [omega]; *)
-(*   try solve [simpl in H0; constructor; apply IHn; eauto; try omega]; *)
-(*   try solve [apply indexr_has in H1; destruct H1; eauto]. *)
-(*   - simpl in H0. *)
-(*     eapply stp_all. *)
-(*     eapply IHn; eauto; try omega. *)
-(*     reflexivity. *)
-(*     assumption. *)
-(*     assumption. *)
-(*     apply IHn; eauto. *)
-(*     simpl. apply closed_open; auto using closed_inc. *)
-(*     unfold open. rewrite <- open_preserves_size. omega. *)
-(*   - remember (open (varH (length GH)) T0) as TT. *)
-(*     assert (stp G (TT :: GH) TT TT). eapply IHn. subst. *)
-(*     eapply closed_open. simpl. eapply closed_upgrade_free. eassumption. omega. *)
-(*     constructor. simpl. omega. subst. unfold open. erewrite <- open_preserves_size. simpl in H0. omega. *)
-(*     eapply stp_bindx; try eassumption. *)
-(*   - simpl in *. assert (stp G GH T1 T1). eapply IHn; try eassumption; try omega. *)
-(*     assert (stp G GH T2 T2). eapply IHn; try eassumption; try omega. *)
-(*     eapply stp_and2; try eassumption. econstructor; try eassumption. eapply stp_and12; try eassumption. *)
-(* Qed. *)
-
-(* Lemma stp_refl: forall T G GH, *)
-(*   closed 0 (length GH) (length G) T -> *)
-(*   stp G GH T T. *)
-(* Proof. *)
-(*   intros. apply stp_refl_aux with (n:=S (tsize_flat T)); eauto. *)
-(* Qed. *)
-
-
-(* Lemma concat_same_length: forall {X} (GU: list X) (GL: list X) (GH1: list X) (GH0: list X), *)
-(*   GU ++ GL = GH1 ++ GH0 -> *)
-(*   length GU = length GH1 -> *)
-(*   GU=GH1 /\ GL=GH0. *)
-(* Proof. *)
-(*   intros. generalize dependent GH1. induction GU; intros. *)
-(*   - simpl in H0. induction GH1. rewrite app_nil_l in H. rewrite app_nil_l in H. *)
-(*     split. reflexivity. apply H. *)
-(*     simpl in H0. omega. *)
-(*   - simpl in H0. induction GH1. simpl in H0. omega. *)
-(*     simpl in H0. inversion H0. simpl in H. inversion H. specialize (IHGU GH1 H4 H2). *)
-(*     destruct IHGU. subst. split; reflexivity. *)
-(* Qed. *)
-
-(* Lemma concat_same_length': forall {X} (GU: list X) (GL: list X) (GH1: list X) (GH0: list X), *)
-(*   GU ++ GL = GH1 ++ GH0 -> *)
-(*   length GL = length GH0 -> *)
-(*   GU=GH1 /\ GL=GH0. *)
-(* Proof. *)
-(*   intros. *)
-(*   assert (length (GU ++ GL) = length (GH1 ++ GH0)) as A. { *)
-(*     rewrite H. reflexivity. *)
-(*   } *)
-(*   rewrite app_length in A. rewrite app_length in A. *)
-(*   rewrite H0 in A. apply Nat.add_cancel_r in A. *)
-(*   apply concat_same_length; assumption. *)
-(* Qed. *)
-
-
-(* Lemma indexr_at_index: forall {A} x0 GH0 GH1 (v:A), *)
-(*   beq_nat x0 (length GH1) = true -> *)
-(*   indexr x0 (GH0 ++ v :: GH1) = Some v. *)
-(* Proof. *)
-(*   intros. apply beq_nat_true in H. subst. *)
-(*   induction GH0. *)
-(*   - simpl. rewrite <- beq_nat_refl. reflexivity. *)
-(*   - simpl. *)
-(*     rewrite app_length. simpl. rewrite <- plus_n_Sm. rewrite <- plus_Sn_m. *)
-(*     rewrite false_beq_nat. assumption. omega. *)
-(* Qed. *)
-
-(* Lemma indexr_same: forall {A} x0 (v0:A) GH0 GH1 (v:A) (v':A), *)
-(*   beq_nat x0 (length GH1) = false -> *)
-(*   indexr x0 (GH0 ++ v :: GH1) = Some v0 -> *)
-(*   indexr x0 (GH0 ++ v' :: GH1) = Some v0. *)
-(* Proof. *)
-(*   intros ? ? ? ? ? ? ? E H. *)
-(*   induction GH0. *)
-(*   - simpl. rewrite E. simpl in H. rewrite E in H. apply H. *)
-(*   - simpl. *)
-(*     rewrite app_length. simpl. *)
-(*     case_eq (beq_nat x0 (length GH0 + S (length GH1))); intros E'. *)
-(*     simpl in H. rewrite app_length in H. simpl in H. rewrite E' in H. *)
-(*     rewrite H. reflexivity. *)
-(*     simpl in H. rewrite app_length in H. simpl in H. rewrite E' in H. *)
-(*     rewrite IHGH0. reflexivity. assumption. *)
-(* Qed. *)
-
-(* Inductive venv_ext : venv -> venv -> Prop := *)
-(* | venv_ext_refl : forall G, venv_ext G G *)
-(* | venv_ext_cons : forall T G1 G2, venv_ext G1 G2 -> venv_ext (T::G1) G2. *)
-
-(* Lemma venv_ext__ge_length: *)
-(*   forall G G', *)
-(*     venv_ext G' G -> *)
-(*     length G' >= length G. *)
-(* Proof. *)
-(*   intros. induction H; simpl; omega. *)
-(* Qed. *)
-
-
-(* Lemma indexr_safe_ex: forall H1 GH G1 TF i, *)
-(*              R_env H1 GH G1 -> *)
-(*              indexr i G1 = Some TF -> *)
-(*              exists d v, indexr i H1 = Some v /\ indexr i GH = Some d /\ forall n, val_type GH [] TF n (d n) v. *)
-(* Proof. *)
-(*   intros. destruct H. destruct H2. destruct (H3 i TF H0) as [d [v [E [V G]]]]. *)
-(*   exists d. exists v. split. eauto. split. eauto. intros. eapply unvv. apply (G n).  *)
-(* Qed. *)
-
-
-(* (* ### Substitution for relating static and dynamic semantics ### *) *)
-(* Lemma indexr_hit2 {X}: forall x (B:X) A G, *)
-(*   length G = x -> *)
-(*   B = A -> *)
-(*   indexr x (B::G) = Some A. *)
-(* Proof. *)
-(*   intros. *)
-(*   unfold indexr. *)
-(*   assert (beq_nat x (length G) = true). eapply beq_nat_true_iff. eauto. *)
-(*   rewrite H1. subst. reflexivity. *)
-(* Qed. *)
-
-(* Lemma indexr_miss {X}: forall x (B:X) A G, *)
-(*   indexr x (B::G) = A -> *)
-(*   x <> (length G)  -> *)
-(*   indexr x G = A. *)
-(* Proof. *)
-(*   intros. *)
-(*   unfold indexr in H. *)
-(*   assert (beq_nat x (length G) = false). eapply beq_nat_false_iff. eauto. *)
-(*   rewrite H1 in H. eauto. *)
-(* Qed. *)
-
-(* Lemma indexr_hit {X}: forall x (B:X) A G, *)
-(*   indexr x (B::G) = Some A -> *)
-(*   x = length G -> *)
-(*   B = A. *)
-(* Proof. *)
-(*   intros. *)
-(*   unfold indexr in H. *)
-(*   assert (beq_nat x (length G) = true). eapply beq_nat_true_iff. eauto. *)
-(*   rewrite H1 in H. inversion H. eauto. *)
-(* Qed. *)
-
-(* Lemma indexr_hit0: forall GH (GX0:venv) (TX0:ty), *)
-(*       indexr 0 (GH ++ [(GX0, TX0)]) = *)
-(*       Some (GX0, TX0). *)
-(* Proof. *)
-(*   intros GH. induction GH. *)
-(*   - intros. simpl. eauto. *)
-(*   - intros. simpl. destruct a. simpl. rewrite app_length. simpl. *)
-(*     assert (length GH + 1 = S (length GH)). omega. rewrite H. *)
-(*     eauto. *)
-(* Qed. *)
-
-(* Hint Resolve beq_nat_true_iff. *)
-(* Hint Resolve beq_nat_false_iff. *)
-
-(* Lemma closed_no_open: forall T x i j k, *)
-(*   closed i j k T -> *)
-(*   T = open_rec i x T. *)
-(* Proof. *)
-(*   intros. induction H; intros; eauto; *)
-(*   try solve [compute; compute in IHclosed; rewrite <-IHclosed; auto]; *)
-(*   try solve [compute; compute in IHclosed1; compute in IHclosed2; *)
-(*              rewrite <-IHclosed1; rewrite <-IHclosed2; auto]. *)
-
-(*   Case "TVarB". *)
-(*     unfold open_rec. assert (i <> x0). omega. *)
-(*     apply beq_nat_false_iff in H0. *)
-(*     rewrite H0. auto. *)
-(* Qed. *)
-
-(* Lemma open_subst_commute: forall T2 V j k x i, *)
-(* closed i j k (TSel V) -> *)
-(* (open_rec i (varH x) (subst V T2)) = *)
-(* (subst V (open_rec i (varH (x+1)) T2)). *)
-(* Proof.  *)
-(*   intros T2 TX j k. induction T2; intros; eauto; try destruct v; eauto. *)
-(*   - simpl. rewrite IHT2_1; eauto. rewrite IHT2_2; eauto. *)
-(*     eapply closed_upgrade. eauto. eauto. *)
-(*   - simpl. *)
-(*     case_eq (beq_nat i 0); intros E. *)
-(*     apply beq_nat_true in E. subst. *)
-(*     case_eq (beq_nat i0 0); intros E0. *)
-(*     apply beq_nat_true in E0. subst. *)
-(*     destruct TX; eauto. *)
-(*     simpl. destruct i; eauto. *)
-(*     inversion H; subst. omega. *)
-(*     simpl. reflexivity. *)
-(*     case_eq (beq_nat i0 0); intros E0. *)
-(*     apply beq_nat_true in E0. subst. *)
-(*     simpl. destruct TX; eauto. *)
-(*     case_eq (beq_nat i i0); intros E1. *)
-(*     apply beq_nat_true in E1. subst. *)
-(*     inversion H; subst. omega. *)
-(*     reflexivity. *)
-(*     simpl. reflexivity. *)
-(*   - simpl. *)
-(*     case_eq (beq_nat i i0); intros E. *)
-(*     apply beq_nat_true in E; subst. *)
-(*     simpl. *)
-(*     assert (x+1 <> 0) as A by omega. *)
-(*     eapply beq_nat_false_iff in A. *)
-(*     rewrite A. *)
-(*     assert (x = x + 1 - 1) as B. unfold id. omega. *)
-(*     rewrite <- B. reflexivity. *)
-(*     simpl. reflexivity. *)
-(*   - simpl. rewrite IHT2_1. rewrite IHT2_2. eauto. eauto. eauto. *)
-(*   - simpl. rewrite IHT2. reflexivity. eapply closed_upgrade. eassumption. omega. *)
-(*   - simpl. rewrite IHT2_1. rewrite IHT2_2. reflexivity. assumption. assumption. *)
-(* Qed. *)
-
-(* Lemma closed_no_subst: forall T i k TX, *)
-(*    closed i 0 k T -> *)
-(*    subst TX T = T. *)
-(* Proof. *)
-(*   intros T. induction T; intros; inversion H; simpl; eauto; *)
-(*   try solve [rewrite (IHT i k TX); eauto; try omega]; *)
-(*   try solve [rewrite (IHT1 i k TX); eauto; rewrite (IHT2 (S i) k TX); eauto; try omega]; *)
-(*   try solve [rewrite (IHT1 i k TX); eauto; rewrite (IHT2 i k TX); eauto; try omega]; *)
-(*   try omega. *)
-(*   erewrite IHT. reflexivity. eassumption. *)
-(* Qed. *)
-
-(* Lemma closed_subst: forall i j k V T, closed i (j+1) k T -> closed 0 j k (TSel V) -> closed i j k (subst V T). *)
-(* Proof. *)
-(*   intros. generalize dependent i. *)
-(*   induction T; intros; inversion H; *)
-(*   try econstructor; *)
-(*   try eapply IHT1; eauto; try eapply IHT2; eauto; try eapply IHT; eauto. *)
-
-(*   - Case "TVarH". simpl. *)
-(*     case_eq (beq_nat x 0); intros E. *)
-(*     eapply closed_upgrade. eapply closed_upgrade_free. *)
-(*     eauto. omega. eauto. omega. *)
-(*     econstructor. assert (x > 0). eapply beq_nat_false_iff in E. omega. omega. *)
-(* Qed. *)
-
-(* Lemma closed_nosubst: forall i j k V T, closed i (j+1) k T -> nosubst T -> closed i j k (subst V T). *)
-(* Proof. *)
-(*   intros. generalize dependent i. *)
-(*   induction T; intros; inversion H; *)
-(*   try econstructor; *)
-(*   try eapply IHT1; eauto; try eapply IHT2; eauto; try eapply IHT; eauto; subst; *)
-(*   try inversion H0; eauto. *)
-
-(*   - Case "TVarH". simpl. simpl in H0. unfold id in H0. *)
-(*     assert (beq_nat x 0 = false) as E. apply beq_nat_false_iff. assumption. *)
-(*     rewrite E. *)
-(*     eapply cl_selh. omega. *)
-(* Qed. *)
-
-(* Lemma subst_open_commute_m: forall i j k k' j' V T2, closed (i+1) (j+1) k T2 -> closed 0 j' k' (TSel V) -> *)
-(*     subst V (open_rec i (varH (j+1)) T2) = open_rec i (varH j) (subst V T2). *)
-(* Proof. *)
-(*   intros. *)
-(*   generalize dependent i. generalize dependent j. *)
-(*   induction T2; intros; inversion H; simpl; eauto; subst; *)
-(*   try rewrite IHT2_1; *)
-(*   try rewrite IHT2_2; *)
-(*   try rewrite IHT2; eauto. *)
-(*   - Case "TVarH". simpl. case_eq (beq_nat x 0); intros E. *)
-(*     eapply closed_no_open. eapply closed_upgrade. eauto. omega. *)
-(*     eauto. *)
-(*   - Case "TVarB". simpl. case_eq (beq_nat i x); intros E. *)
-(*     simpl. case_eq (beq_nat (j+1) 0); intros E2. *)
-(*     eapply beq_nat_true_iff in E2. omega. *)
-(*     subst. assert (j+1-1 = j) as A. omega. rewrite A. eauto. *)
-(*     eauto. *)
-(* Qed. *)
-
-(* Lemma subst_open_commute: forall i j k k' V T2, closed (i+1) (j+1) k T2 -> closed 0 0 k' (TSel V) -> *)
-(*     subst V (open_rec i (varH (j+1)) T2) = open_rec i (varH j) (subst V T2). *)
-(* Proof. *)
-(*   intros. eapply subst_open_commute_m; eauto. *)
-(* Qed. *)
-
-(* Lemma subst_open_zero: forall i i' k TX T2, closed i' 0 k T2 -> *)
-(*     subst TX (open_rec i (varH 0) T2) = open_rec i TX T2. *)
-(* Proof. *)
-(*   intros. generalize dependent i'. generalize dependent i. *)
-(*   induction T2; intros; inversion H; simpl; eauto; *)
-(*   try solve [rewrite (IHT2_1 _ i'); eauto; *)
-(*              rewrite (IHT2_2 _ (S i')); eauto; *)
-(*              rewrite (IHT2_2 _ (S i')); eauto]; *)
-(*   try solve [rewrite (IHT2_1 _ i'); eauto; *)
-(*              rewrite (IHT2_2 _ i'); eauto]. *)
-(*   subst. *)
-(*   case_eq (beq_nat x 0); intros E. omega. omega. *)
-(*   case_eq (beq_nat i x); intros E. eauto. eauto. *)
-(*   erewrite IHT2. reflexivity. eassumption. *)
-(* Qed. *)
-
-(* Lemma Forall2_length: forall A B f (G1:list A) (G2:list B), *)
-(*                         Forall2 f G1 G2 -> length G1 = length G2. *)
-(* Proof. *)
-(*   intros. induction H. *)
-(*   eauto. *)
-(*   simpl. eauto. *)
-(* Qed. *)
-
-(* Lemma nosubst_intro: forall i k T, closed i 0 k T -> nosubst T. *)
-(* Proof. *)
-(*   intros. generalize dependent i. *)
-(*   induction T; intros; inversion H; simpl; eauto. *)
-(*   omega. *)
-(* Qed. *)
-
-(* Lemma nosubst_open: forall i V T2, nosubst (TSel V) -> nosubst T2 -> nosubst (open_rec i V T2). *)
-(* Proof. *)
-(*   intros. generalize dependent i. induction T2; intros; *)
-(*   try inversion H0; simpl; eauto; destruct v; eauto. *)
-(*   case_eq (beq_nat i i0); intros E. eauto. eauto. *)
-(* Qed. *)
-
-
-
-
-
-
-(* (* ### Value Typing / Logical Relation for Values ### *) *)
-
-(* (* NOTE: we need more generic internal lemmas, due to contravariance *) *)
-
-(* (* used in valtp_widen *) *)
-(* Lemma valtp_closed: forall T1 df vf GH H1 n, *)
-(*   val_type H1 GH T1 n (df n) vf -> *)
-(*   closed 0 (length GH) (length H1) T1. *)
-(* Proof. *)
-(*   induction T1; intros; destruct vf; *)
-(*   rewrite val_type_unfold in H; try eauto; try contradiction. *)
-(*   - (* fun *) ev; econstructor; assumption. *)
-(*   - (* sel *) destruct v. *)
-(*               remember (indexr i H1) as L; try destruct L as [?|]; try contradiction. *)
-(*               constructor. eapply indexr_max. eauto. *)
-(*               remember (indexr i GH) as L; try destruct L as [?|]; try contradiction. *)
-(*               constructor. eapply indexr_max. eauto.  *)
-(*               inversion H.  *)
-(*   - (* sel *) destruct v. *)
-(*               remember (indexr i H1) as L; try destruct L as [?|]; try contradiction. *)
-(*               constructor. eapply indexr_max. eauto. *)
-(*               remember (indexr i GH) as L; try destruct L as [?|]; try contradiction. *)
-(*               constructor. eapply indexr_max. eauto.  *)
-(*               inversion H.  *)
-(*   - ev. constructor; assumption. *)
-(*   - ev. constructor; assumption. *)
-(*   - ev. constructor; assumption. *)
-(*   - ev. constructor. eapply IHT1_1. eassumption. eapply IHT1_2. eassumption. *)
-(*   - ev. constructor. eapply IHT1_1. eassumption. eapply IHT1_2. eassumption. *)
-(* Qed. *)
+
+
+(* ############################################################ *)
+(* Proofs *)
+(* ############################################################ *)
+
+
+
+(* ## Extension, Regularity ## *)
+
+Lemma wf_length : forall vs gs ts,
+                    R_env vs gs ts ->
+                    (length vs = length ts).
+Proof.
+  intros. induction H. auto.
+Qed.
+
+Lemma wf_length2 : forall vs gs ts,
+                    R_env vs gs ts ->
+                    (length gs = length ts).
+Proof.
+  intros. destruct H. destruct H0. auto.
+Qed.
+
+
+Hint Immediate wf_length.
+
+Lemma indexr_max : forall X vs n (T: X),
+                       indexr n vs = Some T ->
+                       n < length vs.
+Proof.
+  intros X vs. induction vs.
+  - Case "nil". intros. inversion H.
+  - Case "cons".
+    intros. inversion H.
+    case_eq (beq_nat n (length vs)); intros E2.
+    + SSCase "hit".
+      eapply beq_nat_true in E2. subst n. compute. eauto.
+    + SSCase "miss".
+      rewrite E2 in H1.
+      assert (n < length vs). eapply IHvs. apply H1.
+      compute. eauto.
+Qed.
+
+Lemma le_xx : forall a b,
+                       a <= b ->
+                       exists E, le_lt_dec a b = left E.
+Proof. intros.
+  case_eq (le_lt_dec a b). intros. eauto.
+  intros. omega.
+Qed.
+Lemma le_yy : forall a b,
+                       a > b ->
+                       exists E, le_lt_dec a b = right E.
+Proof. intros.
+  case_eq (le_lt_dec a b). intros. omega.
+  intros. eauto.
+Qed.
+
+Lemma indexr_extend : forall X vs n x (T: X),
+                       indexr n vs = Some T ->
+                       indexr n (x::vs) = Some T.
+
+Proof.
+  intros.
+  assert (n < length vs). eapply indexr_max. eauto.
+  assert (beq_nat n (length vs) = false) as E. eapply beq_nat_false_iff. omega.
+  unfold indexr. unfold indexr in H. rewrite H. rewrite E. reflexivity.
+Qed.
+
+(* splicing -- for stp_extend. *)
+
+Fixpoint splice n (T : ty) {struct T} : ty :=
+  match T with
+    | TTop         => TTop
+    | TBot         => TBot
+    | TAll T1 T2   => TAll (splice n T1) (splice n T2)
+    | TSel (varF i) => TSel (varF i)
+    | TSel (varB i) => TSel (varB i)
+    | TSel (varH i) => if le_lt_dec n i then TSel (varH (i+1)) else TSel (varH i)
+    | TMem T1 T2   => TMem (splice n T1) (splice n T2)
+    | TBind T      => TBind (splice n T)
+    | TAnd T1 T2   => TAnd (splice n T1) (splice n T2)
+  end.
+
+Definition spliceat n (V: (venv*ty)) :=
+  match V with
+    | (G,T) => (G,splice n T)
+  end.
+
+Lemma splice_open_permute: forall {X} (G0:list X) T2 n j,
+(open_rec j (varH (n + S (length G0))) (splice (length G0) T2)) =
+(splice (length G0) (open_rec j (varH (n + length G0)) T2)).
+Proof.
+  intros X G T. induction T; intros; simpl; eauto;
+  try rewrite IHT1; try rewrite IHT2; try rewrite IHT; eauto;
+  destruct v; eauto.
+
+  case_eq (le_lt_dec (length G) i); intros E LE; simpl; eauto.
+  rewrite LE. eauto.
+  rewrite LE. eauto.
+  case_eq (beq_nat j i); intros E; simpl; eauto.
+  case_eq (le_lt_dec (length G) (n + length G)); intros EL LE.
+  rewrite E.
+  assert (n + S (length G) = n + length G + 1). omega.
+  rewrite H. eauto.
+  omega.
+  rewrite E. eauto.
+Qed.
+
+Lemma indexr_splice_hi: forall G0 G2 x0 v1 T,
+    indexr x0 (G2 ++ G0) = Some T ->
+    length G0 <= x0 ->
+    indexr (x0 + 1) (map (splice (length G0)) G2 ++ v1 :: G0) = Some (splice (length G0) T).
+Proof.
+  intros G0 G2. induction G2; intros.
+  - eapply indexr_max in H. simpl in H. omega.
+  - simpl in H.
+    case_eq (beq_nat x0 (length (G2 ++ G0))); intros E.
+    + rewrite E in H. inversion H. subst. simpl.
+      rewrite app_length in E.
+      rewrite app_length. rewrite map_length. simpl.
+      assert (beq_nat (x0 + 1) (length G2 + S (length G0)) = true). {
+        eapply beq_nat_true_iff. eapply beq_nat_true_iff in E. omega.
+      }
+      rewrite H1. eauto.
+    + rewrite E in H.  eapply IHG2 in H. eapply indexr_extend. eapply H. eauto.
+Qed.
+
+Lemma indexr_spliceat_hi: forall G0 G2 x0 v1 G T,
+    indexr x0 (G2 ++ G0) = Some (G, T) ->
+    length G0 <= x0 ->
+    indexr (x0 + 1) (map (spliceat (length G0)) G2 ++ v1 :: G0) =
+    Some (G, splice (length G0) T).
+Proof.
+  intros G0 G2. induction G2; intros.
+  - eapply indexr_max in H. simpl in H. omega.
+  - simpl in H. destruct a.
+    case_eq (beq_nat x0 (length (G2 ++ G0))); intros E.
+    + rewrite E in H. inversion H. subst. simpl.
+      rewrite app_length in E.
+      rewrite app_length. rewrite map_length. simpl.
+      assert (beq_nat (x0 + 1) (length G2 + S (length G0)) = true). {
+        eapply beq_nat_true_iff. eapply beq_nat_true_iff in E. omega.
+      }
+      rewrite H1. eauto.
+    + rewrite E in H.  eapply IHG2 in H. eapply indexr_extend. eapply H. eauto.
+Qed.
+
+Lemma plus_lt_contra: forall a b,
+  a + b < b -> False.
+Proof.
+  intros a b H. induction a.
+  - simpl in H. apply lt_irrefl in H. assumption.
+  - simpl in H. apply IHa. omega.
+Qed.
+
+Lemma indexr_splice_lo0: forall {X} G0 G2 x0 (T:X),
+    indexr x0 (G2 ++ G0) = Some T ->
+    x0 < length G0 ->
+    indexr x0 G0 = Some T.
+Proof.
+  intros X G0 G2. induction G2; intros.
+  - simpl in H. apply H.
+  - simpl in H.
+    case_eq (beq_nat x0 (length (G2 ++ G0))); intros E.
+    + eapply beq_nat_true_iff in E. subst.
+      rewrite app_length in H0. apply plus_lt_contra in H0. inversion H0.
+    + rewrite E in H. apply IHG2. apply H. apply H0.
+Qed.
+
+Lemma indexr_extend_mult: forall {X} G0 G2 x0 (T:X),
+    indexr x0 G0 = Some T ->
+    indexr x0 (G2++G0) = Some T.
+Proof.
+  intros X G0 G2. induction G2; intros.
+  - simpl. assumption.
+  - simpl.
+    case_eq (beq_nat x0 (length (G2 ++ G0))); intros E.
+    + eapply beq_nat_true_iff in E.
+      apply indexr_max in H. subst.
+      rewrite app_length in H. apply plus_lt_contra in H. inversion H.
+    + apply IHG2. assumption.
+Qed.
+
+Lemma indexr_splice_lo: forall G0 G2 x0 v1 T f,
+    indexr x0 (G2 ++ G0) = Some T ->
+    x0 < length G0 ->
+    indexr x0 (map (splice f) G2 ++ v1 :: G0) = Some T.
+Proof.
+  intros.
+  assert (indexr x0 G0 = Some T). eapply indexr_splice_lo0; eauto.
+  eapply indexr_extend_mult. eapply indexr_extend. eauto.
+Qed.
+
+Lemma indexr_spliceat_lo: forall G0 G2 x0 v1 G T f,
+    indexr x0 (G2 ++ G0) = Some (G, T) ->
+    x0 < length G0 ->
+    indexr x0 (map (spliceat f) G2 ++ v1 :: G0) = Some (G, T).
+Proof.
+  intros.
+  assert (indexr x0 G0 = Some (G, T)). eapply indexr_splice_lo0; eauto.
+  eapply indexr_extend_mult. eapply indexr_extend. eauto.
+Qed.
+
+Lemma closed_splice: forall i j k T n,
+  closed i j k T ->
+  closed i (S j) k (splice n T).
+Proof.
+  intros. induction H; simpl; eauto.
+  case_eq (le_lt_dec n x); intros E LE.
+  apply cl_selh. omega.
+  apply cl_selh. omega.
+Qed.
+
+Lemma map_splice_length_inc: forall G0 G2 v1,
+   (length (map (splice (length G0)) G2 ++ v1 :: G0)) = (S (length (G2 ++ G0))).
+Proof.
+  intros. rewrite app_length. rewrite map_length. induction G2.
+  - simpl. reflexivity.
+  - simpl. eauto.
+Qed.
+
+Lemma map_spliceat_length_inc: forall G0 G2 v1,
+   (length (map (spliceat (length G0)) G2 ++ v1 :: G0)) = (S (length (G2 ++ G0))).
+Proof.
+  intros. rewrite app_length. rewrite map_length. induction G2.
+  - simpl. reflexivity.
+  - simpl. eauto.
+Qed.
+
+Lemma closed_inc_mult: forall i j k T,
+  closed i j k T ->
+  forall i' j' k',
+  i' >= i -> j' >= j -> k' >= k ->
+  closed i' j' k' T.
+Proof.
+  intros i j k T H. induction H; intros; eauto; try solve [constructor; omega].
+  - apply cl_all. apply IHclosed1; omega. apply IHclosed2; omega.
+  - constructor. apply IHclosed; omega.
+Qed.
+
+Lemma closed_inc: forall i j k T,
+  closed i j k T ->
+  closed i (S j) k T.
+Proof.
+  intros. apply (closed_inc_mult i j k T H i (S j) k); omega.
+Qed.
+
+Lemma closed_splice_idem: forall i j k T n,
+                            closed i j k T ->
+                            n >= j ->
+                            splice n T = T.
+Proof.
+  intros. induction H; eauto.
+  - (* TAll *) simpl.
+    rewrite IHclosed1. rewrite IHclosed2.
+    reflexivity.
+    assumption. assumption.
+  - (* TVarH *) simpl.
+    case_eq (le_lt_dec n x); intros E LE. omega. reflexivity.
+  - (* TMem *) simpl.
+    rewrite IHclosed1. rewrite IHclosed2.
+    reflexivity.
+    assumption. assumption.
+  - simpl. rewrite IHclosed. reflexivity. assumption.
+  - simpl. rewrite IHclosed1. rewrite IHclosed2. reflexivity. assumption. assumption.
+Qed.
+
+Lemma stp_closed : forall G GH T1 T2,
+                     stp G GH T1 T2 ->
+                     closed 0 (length GH) (length G) T1 /\ closed 0 (length GH) (length G) T2.
+Proof.
+  intros. induction H;
+    try solve [repeat ev; split; try inv_mem; eauto using indexr_max].
+Qed.
+
+Lemma stp_closed2 : forall G1 GH T1 T2,
+                       stp G1 GH T1 T2 ->
+                       closed 0 (length GH) (length G1) T2.
+Proof.
+  intros. apply (proj2 (stp_closed G1 GH T1 T2 H)).
+Qed.
+
+Lemma stp_closed1 : forall G1 GH T1 T2,
+                       stp G1 GH T1 T2 ->
+                       closed 0 (length GH) (length G1) T1.
+Proof.
+  intros. apply (proj1 (stp_closed G1 GH T1 T2 H)).
+Qed.
+
+
+Lemma closed_upgrade: forall i j k i' T,
+ closed i j k T ->
+ i' >= i ->
+ closed i' j k T.
+Proof.
+ intros. apply (closed_inc_mult i j k T H i' j k); omega.
+Qed.
+
+Lemma closed_upgrade_free: forall i j k j' T,
+ closed i j k T ->
+ j' >= j ->
+ closed i j' k T.
+Proof.
+ intros. apply (closed_inc_mult i j k T H i j' k); omega.
+Qed.
+
+Lemma closed_upgrade_freef: forall i j k k' T,
+ closed i j k T ->
+ k' >= k ->
+ closed i j k' T.
+Proof.
+ intros. apply (closed_inc_mult i j k T H i j k'); omega.
+Qed.
+
+Lemma closed_open: forall i j k V T, closed (i+1) j k T -> closed i j k (TSel V) ->
+  closed i j k (open_rec i V T).
+Proof.
+  intros. generalize dependent i.
+  induction T; intros; inversion H;
+  try econstructor;
+  try eapply IHT1; eauto; try eapply IHT2; eauto; try eapply IHT; eauto.
+  eapply closed_upgrade. eauto. eauto.
+  - Case "TVarB". simpl.
+    case_eq (beq_nat i x); intros E. eauto.
+    econstructor. eapply beq_nat_false_iff in E. omega.
+  - eapply closed_upgrade. eassumption. omega.
+Qed.
+
+Lemma indexr_has: forall X (G: list X) x,
+  length G > x ->
+  exists v, indexr x G = Some v.
+Proof.
+  intros. remember (length G) as n.
+  generalize dependent x.
+  generalize dependent G.
+  induction n; intros; try omega.
+  destruct G; simpl.
+  - simpl in Heqn. inversion Heqn.
+  - simpl in Heqn. inversion Heqn. subst.
+    case_eq (beq_nat x (length G)); intros E.
+    + eexists. reflexivity.
+    + apply beq_nat_false in E. apply IHn; eauto.
+      omega.
+Qed.
+
+Lemma stp_refl_aux: forall n T G GH,
+  closed 0 (length GH) (length G) T ->
+  tsize_flat T < n ->
+  stp G GH T T.
+Proof.
+  intros n. induction n; intros; try omega.
+  inversion H; subst; eauto;
+  try solve [omega];
+  try solve [simpl in H0; constructor; apply IHn; eauto; try omega];
+  try solve [apply indexr_has in H1; destruct H1; eauto].
+  - simpl in H0.
+    eapply stp_all.
+    eapply IHn; eauto; try omega.
+    reflexivity.
+    assumption.
+    assumption.
+    apply IHn; eauto.
+    simpl. apply closed_open; auto using closed_inc.
+    unfold open. rewrite <- open_preserves_size. omega.
+  - remember (open (varH (length GH)) T0) as TT.
+    assert (stp G (TT :: GH) TT TT). eapply IHn. subst.
+    eapply closed_open. simpl. eapply closed_upgrade_free. eassumption. omega.
+    constructor. simpl. omega. subst. unfold open. erewrite <- open_preserves_size. simpl in H0. omega.
+    eapply stp_bindx; try eassumption.
+  - simpl in *. assert (stp G GH T1 T1). eapply IHn; try eassumption; try omega.
+    assert (stp G GH T2 T2). eapply IHn; try eassumption; try omega.
+    eapply stp_and2; try eassumption. econstructor; try eassumption. eapply stp_and12; try eassumption.
+Qed.
+
+Lemma stp_refl: forall T G GH,
+  closed 0 (length GH) (length G) T ->
+  stp G GH T T.
+Proof.
+  intros. apply stp_refl_aux with (n:=S (tsize_flat T)); eauto.
+Qed.
+
+
+Lemma concat_same_length: forall {X} (GU: list X) (GL: list X) (GH1: list X) (GH0: list X),
+  GU ++ GL = GH1 ++ GH0 ->
+  length GU = length GH1 ->
+  GU=GH1 /\ GL=GH0.
+Proof.
+  intros. generalize dependent GH1. induction GU; intros.
+  - simpl in H0. induction GH1. rewrite app_nil_l in H. rewrite app_nil_l in H.
+    split. reflexivity. apply H.
+    simpl in H0. omega.
+  - simpl in H0. induction GH1. simpl in H0. omega.
+    simpl in H0. inversion H0. simpl in H. inversion H. specialize (IHGU GH1 H4 H2).
+    destruct IHGU. subst. split; reflexivity.
+Qed.
+
+Lemma concat_same_length': forall {X} (GU: list X) (GL: list X) (GH1: list X) (GH0: list X),
+  GU ++ GL = GH1 ++ GH0 ->
+  length GL = length GH0 ->
+  GU=GH1 /\ GL=GH0.
+Proof.
+  intros.
+  assert (length (GU ++ GL) = length (GH1 ++ GH0)) as A. {
+    rewrite H. reflexivity.
+  }
+  rewrite app_length in A. rewrite app_length in A.
+  rewrite H0 in A. apply Nat.add_cancel_r in A.
+  apply concat_same_length; assumption.
+Qed.
+
+
+Lemma indexr_at_index: forall {A} x0 GH0 GH1 (v:A),
+  beq_nat x0 (length GH1) = true ->
+  indexr x0 (GH0 ++ v :: GH1) = Some v.
+Proof.
+  intros. apply beq_nat_true in H. subst.
+  induction GH0.
+  - simpl. rewrite <- beq_nat_refl. reflexivity.
+  - simpl.
+    rewrite app_length. simpl. rewrite <- plus_n_Sm. rewrite <- plus_Sn_m.
+    rewrite false_beq_nat. assumption. omega.
+Qed.
+
+Lemma indexr_same: forall {A} x0 (v0:A) GH0 GH1 (v:A) (v':A),
+  beq_nat x0 (length GH1) = false ->
+  indexr x0 (GH0 ++ v :: GH1) = Some v0 ->
+  indexr x0 (GH0 ++ v' :: GH1) = Some v0.
+Proof.
+  intros ? ? ? ? ? ? ? E H.
+  induction GH0.
+  - simpl. rewrite E. simpl in H. rewrite E in H. apply H.
+  - simpl.
+    rewrite app_length. simpl.
+    case_eq (beq_nat x0 (length GH0 + S (length GH1))); intros E'.
+    simpl in H. rewrite app_length in H. simpl in H. rewrite E' in H.
+    rewrite H. reflexivity.
+    simpl in H. rewrite app_length in H. simpl in H. rewrite E' in H.
+    rewrite IHGH0. reflexivity. assumption.
+Qed.
+
+Inductive venv_ext : venv -> venv -> Prop :=
+| venv_ext_refl : forall G, venv_ext G G
+| venv_ext_cons : forall T G1 G2, venv_ext G1 G2 -> venv_ext (T::G1) G2.
+
+Lemma venv_ext__ge_length:
+  forall G G',
+    venv_ext G' G ->
+    length G' >= length G.
+Proof.
+  intros. induction H; simpl; omega.
+Qed.
+
+
+Lemma indexr_safe_ex: forall H1 GH G1 TF i,
+             R_env H1 GH G1 ->
+             indexr i G1 = Some TF ->
+             exists v, indexr i H1 = Some v /\ forall n, val_type GH [] TF n v.
+Proof.
+  intros. destruct H. destruct H2. destruct (H3 i TF H0) as [v [E G]].
+  exists v. split. eauto. intros. eapply unvv. apply (G n).
+Qed.
+
+
+(* ### Substitution for relating static and dynamic semantics ### *)
+Lemma indexr_hit2 {X}: forall x (B:X) A G,
+  length G = x ->
+  B = A ->
+  indexr x (B::G) = Some A.
+Proof.
+  intros.
+  unfold indexr.
+  assert (beq_nat x (length G) = true). eapply beq_nat_true_iff. eauto.
+  rewrite H1. subst. reflexivity.
+Qed.
+
+Lemma indexr_miss {X}: forall x (B:X) A G,
+  indexr x (B::G) = A ->
+  x <> (length G)  ->
+  indexr x G = A.
+Proof.
+  intros.
+  unfold indexr in H.
+  assert (beq_nat x (length G) = false). eapply beq_nat_false_iff. eauto.
+  rewrite H1 in H. eauto.
+Qed.
+
+Lemma indexr_hit {X}: forall x (B:X) A G,
+  indexr x (B::G) = Some A ->
+  x = length G ->
+  B = A.
+Proof.
+  intros.
+  unfold indexr in H.
+  assert (beq_nat x (length G) = true). eapply beq_nat_true_iff. eauto.
+  rewrite H1 in H. inversion H. eauto.
+Qed.
+
+Lemma indexr_hit0: forall GH (GX0:venv) (TX0:ty),
+      indexr 0 (GH ++ [(GX0, TX0)]) =
+      Some (GX0, TX0).
+Proof.
+  intros GH. induction GH.
+  - intros. simpl. eauto.
+  - intros. simpl. destruct a. simpl. rewrite app_length. simpl.
+    assert (length GH + 1 = S (length GH)). omega. rewrite H.
+    eauto.
+Qed.
+
+Hint Resolve beq_nat_true_iff.
+Hint Resolve beq_nat_false_iff.
+
+Lemma closed_no_open: forall T x i j k,
+  closed i j k T ->
+  T = open_rec i x T.
+Proof.
+  intros. induction H; intros; eauto;
+  try solve [compute; compute in IHclosed; rewrite <-IHclosed; auto];
+  try solve [compute; compute in IHclosed1; compute in IHclosed2;
+             rewrite <-IHclosed1; rewrite <-IHclosed2; auto].
+
+  Case "TVarB".
+    unfold open_rec. assert (i <> x0). omega.
+    apply beq_nat_false_iff in H0.
+    rewrite H0. auto.
+Qed.
+
+Lemma open_subst_commute: forall T2 V j k x i,
+closed i j k (TSel V) ->
+(open_rec i (varH x) (subst V T2)) =
+(subst V (open_rec i (varH (x+1)) T2)).
+Proof.
+  intros T2 TX j k. induction T2; intros; eauto; try destruct v; eauto.
+  - simpl. rewrite IHT2_1; eauto. rewrite IHT2_2; eauto.
+    eapply closed_upgrade. eauto. eauto.
+  - simpl.
+    case_eq (beq_nat i 0); intros E.
+    apply beq_nat_true in E. subst.
+    case_eq (beq_nat i0 0); intros E0.
+    apply beq_nat_true in E0. subst.
+    destruct TX; eauto.
+    simpl. destruct i; eauto.
+    inversion H; subst. omega.
+    simpl. reflexivity.
+    case_eq (beq_nat i0 0); intros E0.
+    apply beq_nat_true in E0. subst.
+    simpl. destruct TX; eauto.
+    case_eq (beq_nat i i0); intros E1.
+    apply beq_nat_true in E1. subst.
+    inversion H; subst. omega.
+    reflexivity.
+    simpl. reflexivity.
+  - simpl.
+    case_eq (beq_nat i i0); intros E.
+    apply beq_nat_true in E; subst.
+    simpl.
+    assert (x+1 <> 0) as A by omega.
+    eapply beq_nat_false_iff in A.
+    rewrite A.
+    assert (x = x + 1 - 1) as B. unfold id. omega.
+    rewrite <- B. reflexivity.
+    simpl. reflexivity.
+  - simpl. rewrite IHT2_1. rewrite IHT2_2. eauto. eauto. eauto.
+  - simpl. rewrite IHT2. reflexivity. eapply closed_upgrade. eassumption. omega.
+  - simpl. rewrite IHT2_1. rewrite IHT2_2. reflexivity. assumption. assumption.
+Qed.
+
+Lemma closed_no_subst: forall T i k TX,
+   closed i 0 k T ->
+   subst TX T = T.
+Proof.
+  intros T. induction T; intros; inversion H; simpl; eauto;
+  try solve [rewrite (IHT i k TX); eauto; try omega];
+  try solve [rewrite (IHT1 i k TX); eauto; rewrite (IHT2 (S i) k TX); eauto; try omega];
+  try solve [rewrite (IHT1 i k TX); eauto; rewrite (IHT2 i k TX); eauto; try omega];
+  try omega.
+  erewrite IHT. reflexivity. eassumption.
+Qed.
+
+Lemma closed_subst: forall i j k V T, closed i (j+1) k T -> closed 0 j k (TSel V) -> closed i j k (subst V T).
+Proof.
+  intros. generalize dependent i.
+  induction T; intros; inversion H;
+  try econstructor;
+  try eapply IHT1; eauto; try eapply IHT2; eauto; try eapply IHT; eauto.
+
+  - Case "TVarH". simpl.
+    case_eq (beq_nat x 0); intros E.
+    eapply closed_upgrade. eapply closed_upgrade_free.
+    eauto. omega. eauto. omega.
+    econstructor. assert (x > 0). eapply beq_nat_false_iff in E. omega. omega.
+Qed.
+
+Lemma closed_nosubst: forall i j k V T, closed i (j+1) k T -> nosubst T -> closed i j k (subst V T).
+Proof.
+  intros. generalize dependent i.
+  induction T; intros; inversion H;
+  try econstructor;
+  try eapply IHT1; eauto; try eapply IHT2; eauto; try eapply IHT; eauto; subst;
+  try inversion H0; eauto.
+
+  - Case "TVarH". simpl. simpl in H0. unfold id in H0.
+    assert (beq_nat x 0 = false) as E. apply beq_nat_false_iff. assumption.
+    rewrite E.
+    eapply cl_selh. omega.
+Qed.
+
+Lemma subst_open_commute_m: forall i j k k' j' V T2, closed (i+1) (j+1) k T2 -> closed 0 j' k' (TSel V) ->
+    subst V (open_rec i (varH (j+1)) T2) = open_rec i (varH j) (subst V T2).
+Proof.
+  intros.
+  generalize dependent i. generalize dependent j.
+  induction T2; intros; inversion H; simpl; eauto; subst;
+  try rewrite IHT2_1;
+  try rewrite IHT2_2;
+  try rewrite IHT2; eauto.
+  - Case "TVarH". simpl. case_eq (beq_nat x 0); intros E.
+    eapply closed_no_open. eapply closed_upgrade. eauto. omega.
+    eauto.
+  - Case "TVarB". simpl. case_eq (beq_nat i x); intros E.
+    simpl. case_eq (beq_nat (j+1) 0); intros E2.
+    eapply beq_nat_true_iff in E2. omega.
+    subst. assert (j+1-1 = j) as A. omega. rewrite A. eauto.
+    eauto.
+Qed.
+
+Lemma subst_open_commute: forall i j k k' V T2, closed (i+1) (j+1) k T2 -> closed 0 0 k' (TSel V) ->
+    subst V (open_rec i (varH (j+1)) T2) = open_rec i (varH j) (subst V T2).
+Proof.
+  intros. eapply subst_open_commute_m; eauto.
+Qed.
+
+Lemma subst_open_zero: forall i i' k TX T2, closed i' 0 k T2 ->
+    subst TX (open_rec i (varH 0) T2) = open_rec i TX T2.
+Proof.
+  intros. generalize dependent i'. generalize dependent i.
+  induction T2; intros; inversion H; simpl; eauto;
+  try solve [rewrite (IHT2_1 _ i'); eauto;
+             rewrite (IHT2_2 _ (S i')); eauto;
+             rewrite (IHT2_2 _ (S i')); eauto];
+  try solve [rewrite (IHT2_1 _ i'); eauto;
+             rewrite (IHT2_2 _ i'); eauto].
+  subst.
+  case_eq (beq_nat x 0); intros E. omega. omega.
+  case_eq (beq_nat i x); intros E. eauto. eauto.
+  erewrite IHT2. reflexivity. eassumption.
+Qed.
+
+Lemma Forall2_length: forall A B f (G1:list A) (G2:list B),
+                        Forall2 f G1 G2 -> length G1 = length G2.
+Proof.
+  intros. induction H.
+  eauto.
+  simpl. eauto.
+Qed.
+
+Lemma nosubst_intro: forall i k T, closed i 0 k T -> nosubst T.
+Proof.
+  intros. generalize dependent i.
+  induction T; intros; inversion H; simpl; eauto.
+  omega.
+Qed.
+
+Lemma nosubst_open: forall i V T2, nosubst (TSel V) -> nosubst T2 -> nosubst (open_rec i V T2).
+Proof.
+  intros. generalize dependent i. induction T2; intros;
+  try inversion H0; simpl; eauto; destruct v; eauto.
+  case_eq (beq_nat i i0); intros E. eauto. eauto.
+Qed.
+
+
+
+
+
+
+(* ### Value Typing / Logical Relation for Values ### *)
+
+(* NOTE: we need more generic internal lemmas, due to contravariance *)
+
+(* used in valtp_widen *)
+Lemma valtp_closed: forall T1 vf GH H1 n,
+  vtp H1 GH T1 n  vf ->
+  closed 0 (length GH) (length H1) T1.
+Proof.
+  induction T1; intros; destruct vf;
+  rewrite val_type_unfold in H; try eauto; try contradiction.
+  - (* fun *) ev; econstructor; assumption.
+  - (* sel *) destruct v.
+              remember (indexr i H1) as L; try destruct L as [?|]; try contradiction.
+              constructor. eapply indexr_max. eauto.
+              remember (indexr i GH) as L; try destruct L as [?|]; try contradiction.
+              constructor. eapply indexr_max. eauto.
+              inversion H.
+  - (* sel *) destruct v.
+              remember (indexr i H1) as L; try destruct L as [?|]; try contradiction.
+              constructor. eapply indexr_max. eauto.
+              remember (indexr i GH) as L; try destruct L as [?|]; try contradiction.
+              constructor. eapply indexr_max. eauto.
+              inversion H.
+  - ev. constructor; assumption.
+  - ev. constructor; assumption.
+  - ev. constructor; assumption.
+  - ev. constructor. eapply IHT1_1. eassumption. eapply IHT1_2. eassumption.
+  - ev. constructor. eapply IHT1_1. eassumption. eapply IHT1_2. eassumption.
+Qed.
 
  
-(* Lemma valtp_extend_aux: forall n T1 vx vf df k H1 G1, *)
-(*   tsize_flat T1 < n -> *)
-(*   closed 0 (length G1) (length H1) T1 -> *)
-(*   (vtp H1 G1 T1 k (df k) vf <-> vtp (vx :: H1) G1 T1 k (df k) vf). *)
-(* Proof. *)
-(*   induction n; intros ? ? ? ? ? ? ? S C. inversion S. *)
-(*   destruct T1; split; intros V; apply unvv in V; rewrite val_type_unfold in V. *)
-(*   - apply vv. rewrite val_type_unfold. assumption. *)
-(*   - apply vv. rewrite val_type_unfold. assumption. *)
-(*   - apply vv. rewrite val_type_unfold. assumption. *)
-(*   - apply vv. rewrite val_type_unfold. assumption. *)
-(*   - destruct vf; try solve [inversion V]. ev. *)
-(*     apply vv. rewrite val_type_unfold.  *)
-(*     split. simpl. eapply closed_upgrade_freef. apply H. omega. *)
-(*     split. simpl. eapply closed_upgrade_freef. apply H0. omega.  *)
-(*     intros. *)
-(*     assert (forall kx: nat, val_type (H1) G1 T1_1 kx (jj kx) vx0). *)
-(*     intros. simpl in S. assert (tsize_flat T1_1 < n). omega.  *)
-(*     apply unvv. eapply IHn with (H1 := H1); simpl; try apply vv; try eassumption; auto. *)
-(*     specialize (H2 _ _ H4). ev. exists x. exists x0. split. assumption. intros.  *)
-(*     apply unvv. eapply IHn with (H1 := H1). unfold open. rewrite <-open_preserves_size. *)
-(*     simpl in S. omega.  *)
-(*     eapply closed_open. simpl. eapply closed_upgrade_free. eassumption. omega. *)
-(*     constructor. simpl. omega. apply vv. auto. *)
+Lemma valtp_extend_aux: forall n T1 vx vf k H1 G1,
+  tsize_flat T1 < n ->
+  closed 0 (length G1) (length H1) T1 ->
+  (vtp H1 G1 T1 k vf <-> vtp (vx :: H1) G1 T1 k vf).
+Proof.
+  induction n; intros ? ? ? ? ? ? S C. inversion S.
+  destruct T1; split; intros V; rewrite val_type_unfold in V.
+  - rewrite val_type_unfold. assumption.
+  - rewrite val_type_unfold. assumption.
+  - rewrite val_type_unfold. assumption.
+  - rewrite val_type_unfold. assumption.
+  - destruct vf; try solve [inversion V]. ev.
+    rewrite val_type_unfold.
+    split. simpl. eapply closed_upgrade_freef. apply H. omega.
+    split. simpl. eapply closed_upgrade_freef. apply H0. omega.
+    intros.
+    assert (vtp (H1) G1 T1_1 j vx0).
+    intros. simpl in S. assert (tsize_flat T1_1 < n) by omega.
+    eapply IHn with (H1 := H1); simpl; try apply vv; try eassumption; auto.
+    apply unvv.
+    apply H3.
+    (* assert (forall jx: nat, jx < k -> val_type (H1) G1 T1_1 jx vx0). *)
+    (* intros. simpl in S. assert (tsize_flat T1_1 < n) by omega. *)
+    (* apply unvv. eapply IHn with (H1 := H1); simpl; try apply vv; try eassumption; auto. *)
+    (* apply unvv. *)
+    (* apply H3. *)
+    specialize (H2 _ j Hj H4).
+    ev. exists x. split. assumption.
+    eapply IHn with (H1 := H1). unfold open. rewrite <-open_preserves_size.
+    simpl in S. omega.
+    eapply closed_open. simpl. eapply closed_upgrade_free. eassumption. omega.
+    constructor. simpl. omega.
+    assumption.
+  - destruct vf; try solve by inversion. ev.
+    rewrite val_type_unfold. inversion C. subst.
+    split. assumption. split. assumption. intros.
+    assert (vtp (vx :: H1) G1 T1_1 j vx0).
+    intros. eapply IHn with (H1 := H1). simpl in S. omega. assumption.
+    assumption.
+    specialize (H2 _ j Hj H4).
+    ev. exists x. split. assumption. eapply IHn with (H1 := H1).
+    unfold open. rewrite <- open_preserves_size. simpl in S. omega.
+    eapply closed_open. simpl. eapply closed_upgrade_free. eassumption. omega.
+    constructor. simpl. omega.
+    eapply H5.
 
-(*   - destruct vf; try solve by inversion. ev.  *)
-(*     apply vv. rewrite val_type_unfold. inversion C. subst. *)
-(*     split. assumption. split. assumption. intros. *)
-(*     assert (forall kx : nat, val_type (vx :: H1) G1 T1_1 kx (jj kx) vx0). *)
-(*     intros. apply unvv. eapply IHn with (H1 := H1). simpl in S. omega. assumption.  *)
-(*     apply vv. auto.  *)
-(*     specialize (H2 _ _ H4). *)
-(*     ev. exists x. exists x0. split. assumption. intros. apply unvv. eapply IHn with (H1 := H1). *)
-(*     unfold open. rewrite <- open_preserves_size. simpl in S. omega. *)
-(*     eapply closed_open. simpl. eapply closed_upgrade_free. eassumption. omega. *)
-(*     constructor. simpl. omega. *)
-(*     apply vv. eapply H5. *)
+  - rewrite val_type_unfold. destruct vf.
+    + destruct v.
+    destruct (indexr i H1) eqn : A.
+    assert (indexr i (vx :: H1) = Some v). apply indexr_extend. assumption. rewrite H. assumption.
+    inversion V. assumption. inversion V.
+    + destruct v.
+    destruct (indexr i H1) eqn : A.
+    assert (indexr i (vx :: H1) = Some v). apply indexr_extend. assumption. rewrite H. assumption.
+    inversion V. assumption. inversion V.
 
-(*   - apply vv. rewrite val_type_unfold. destruct vf. *)
-(*     + destruct v. *)
-(*     destruct (indexr i H1) eqn : A. *)
-(*     assert (indexr i (vx :: H1) = Some v). apply indexr_extend. assumption. rewrite H. assumption. *)
-(*     inversion V. assumption. inversion V.  *)
-(*     + destruct v. *)
-(*     destruct (indexr i H1) eqn : A.  *)
-(*     assert (indexr i (vx :: H1) = Some v). apply indexr_extend. assumption. rewrite H. assumption. *)
-(*     inversion V. assumption. inversion V. *)
+  - rewrite val_type_unfold. destruct vf.
+    + destruct v. inversion C. subst.
+    eapply indexr_has in H4. ev. assert (indexr i (vx:: H1) = Some x). apply indexr_extend.
+    assumption. rewrite H0 in V. rewrite H. assumption. assumption. inversion V.
+    + destruct v. inversion C. subst.
+    eapply indexr_has in H4. ev. assert (indexr i (vx:: H1) = Some x). apply indexr_extend.
+    assumption. rewrite H0 in V. rewrite H. assumption. assumption. inversion V.
 
-(*   - apply vv. rewrite val_type_unfold. destruct vf. *)
-(*     + destruct v. inversion C. subst.  *)
-(*     eapply indexr_has in H4. ev. assert (indexr i (vx:: H1) = Some x). apply indexr_extend. *)
-(*     assumption. rewrite H0 in V. rewrite H. assumption. assumption. inversion V. *)
-(*     + destruct v. inversion C. subst.  *)
-(*     eapply indexr_has in H4. ev. assert (indexr i (vx:: H1) = Some x). apply indexr_extend. *)
-(*     assumption. rewrite H0 in V. rewrite H. assumption. assumption. inversion V. *)
+  - inversion C. subst. rewrite val_type_unfold. destruct vf; try solve by inversion.
+    ev.
+    repeat split_conj.
 
-(*   - inversion C. subst. apply vv. rewrite val_type_unfold. destruct vf; try solve by inversion. *)
-(*     ev. split. simpl. eapply closed_upgrade_freef. eassumption. omega. *)
-(*         split. simpl. eapply closed_upgrade_freef. eassumption. omega. *)
-(*         destruct k. auto. intros. specialize (H2 dy vy). ev. split. *)
-(*         intros. apply H2. apply unvv. eapply IHn. simpl in S. omega. assumption. apply vv. eassumption. *)
-(*         intros. specialize (H3 H4). apply unvv. eapply IHn with (H1 := H1). simpl in S. omega. *)
-(*         assumption. apply vv. assumption. *)
+    + simpl. eapply closed_upgrade_freef. eassumption. omega.
+    + simpl. eapply closed_upgrade_freef. eassumption. omega.
+    + intros.
+      simpl in S.
+      assert (tsize_flat T1_1 + tsize_flat T1_2 < n) by omega.
+      specialize (H2 j Hj vy). ev.
+      split; intros.
+      * apply H2.
+        eapply IHn with (H1 := H1); omega || eauto.
+      * eapply IHn with (H1 := H1); omega || eauto.
 
-(*   - inversion C. subst. apply vv. rewrite val_type_unfold. destruct vf; try solve by inversion. *)
-(*     ev. destruct k. repeat split; try assumption. *)
-(*     split. assumption. split. assumption. intros. specialize (H2 dy vy). ev. *)
-(*     split. intros. apply H2. apply unvv. eapply IHn with (H1:= H1). simpl in S. omega. assumption. *)
-(*     apply vv. assumption. intros. specialize (H3 H4). apply unvv. eapply IHn with (H1 := H1). simpl in S. omega. *)
-(*     assumption. apply vv. eassumption. *)
+        (* destruct k. auto. intros. specialize (H2 vy). ev. split. *)
+        (* intros. apply H2. apply unvv. eapply IHn. simpl in S. omega. assumption. apply vv. eassumption. *)
+        (* intros. specialize (H3 H4). apply unvv. eapply IHn with (H1 := H1). simpl in S. omega. *)
+        (* assumption. apply vv. assumption. *)
 
-(*   - inversion C. subst. simpl in *. apply vv. rewrite val_type_unfold. *)
-(*     assert (closed 1 (length G1) (length H1) T1 /\ *)
-(*         (exists jj : forall x : nat, vset x, *)
-(*            jj k = df k /\ *)
-(*            (forall n0 : nat, *)
-(*             val_type H1 (jj :: G1) (open (varH (length G1)) T1) n0 (jj n0) vf))). destruct vf; assumption. clear V. ev. *)
-(*     assert (closed 1 (length G1) (length (vx :: H1)) T1 /\ *)
-(*     (exists jj : forall x0 : nat, vset x0, *)
-(*        jj k = df k /\ *)
-(*        (forall n0 : nat, *)
-(*         val_type (vx :: H1) (jj :: G1) (open (varH (length G1)) T1) n0 *)
-(*           (jj n0) vf))) as Goal. *)
-(*     split. simpl. eapply closed_upgrade_freef. eassumption. omega. *)
-(*     exists x. split. assumption. intros. specialize (H2 n0). apply unvv. eapply IHn with (H1 := H1). *)
-(*     unfold open. rewrite <- open_preserves_size. omega.  *)
-(*     eapply closed_open. simpl. eapply closed_upgrade_free. eassumption. omega.  *)
-(*     constructor. simpl. omega. *)
-(*     apply vv. assumption. *)
-(*     destruct vf; apply Goal. *)
+  - inversion C. subst. rewrite val_type_unfold. destruct vf; try solve by inversion.
+    ev.
+    simpl in S.
+    assert (tsize_flat T1_1 + tsize_flat T1_2 < n) by omega.
+    repeat split_conj; try assumption; intros.
+    
+    (* destruct k. repeat split; try assumption. *)
+    (* split. assumption. split. assumption. *)
+    specialize (H2 j Hj vy). ev.
+    split; intros.
+    + apply H2.
+      eapply IHn with (H1:= H1); omega || assumption.
+    +
+      eapply IHn with (H1:= H1); omega || auto.
 
-(*   - inversion C. subst. apply vv. rewrite val_type_unfold.  *)
-(*     assert (closed 1 (length G1) (length (vx :: H1)) T1 /\ *)
-(*         (exists jj : forall x : nat, vset x, *)
-(*            jj k = df k /\ *)
-(*            (forall n0 : nat, *)
-(*             val_type (vx :: H1) (jj :: G1) (open (varH (length G1)) T1) n0 *)
-(*               (jj n0) vf))). destruct vf; assumption. clear V. ev. *)
-(*     assert (closed 1 (length G1) (length H1) T1 /\ *)
-(*     (exists jj : forall x0 : nat, vset x0, *)
-(*        jj k = df k /\ *)
-(*        (forall n0 : nat, *)
-(*         val_type H1 (jj :: G1) (open (varH (length G1)) T1) n0 (jj n0) vf))) as Goal.  *)
-(*     split. assumption. exists x. split. assumption. intros. specialize (H2 n0). *)
-(*     apply unvv. eapply IHn with (H1 := H1). unfold open. rewrite <- open_preserves_size. *)
-(*     simpl in S. omega. eapply closed_open. simpl. eapply closed_upgrade_free. eassumption. omega. *)
-(*     constructor. simpl. omega. apply vv. eassumption. *)
-(*     destruct vf; apply Goal. *)
+  - inversion C. subst.
+    simpl in *.
+    assert (tsize_flat T1 < n) by omega.
+    rewrite val_type_unfold.
+    match_case_analysis; ev; repeat split_conj; simpl.
+    + eapply closed_upgrade_freef; eassumption || omega.
+    + intros.
+      eapply IHn with (H1 := H1); try eassumption || omega.
+      * unfold open. rewrite <- open_preserves_size. omega.
+      * eapply closed_open. simpl. eapply closed_upgrade_free.
+        eassumption.
+        all: omega || constructor; simpl; omega.
+      * eapply H2; assumption.
+    + eapply closed_upgrade_freef. eassumption. omega.
 
-(*   - inversion C. subst. simpl in *. apply vv. rewrite val_type_unfold.  *)
-(*     destruct vf. ev. *)
-(*     split. apply unvv. apply vv in H. eapply IHn with (H1 := H1); try eassumption; try omega. *)
-(*     apply unvv. apply vv in H0. eapply IHn with (H1 := H1); try eassumption; try omega. *)
-(*     ev. *)
-(*     split. apply unvv. apply vv in H. eapply IHn with (H1 := H1); try eassumption; try omega. *)
-(*     apply unvv. apply vv in H0. eapply IHn with (H1 := H1); try eassumption; try omega. *)
-(*   - inversion C. subst. simpl in *. apply vv. rewrite val_type_unfold.  *)
-(*     destruct vf. ev. *)
-(*     split. apply unvv. apply vv in H. eapply IHn with (H1 := H1); try eassumption; try omega. *)
-(*     apply unvv. apply vv in H0. eapply IHn with (H1 := H1); try eassumption; try omega. *)
-(*     ev.  *)
-(*     split. apply unvv. apply vv in H. eapply IHn with (H1 := H1); try eassumption; try omega. *)
-(*     apply unvv. apply vv in H0. eapply IHn with (H1 := H1); try eassumption; try omega. *)
-(* Qed. *)
+    + intros.
+      (* eapply IHn with (H1 := H1). *)
+      (* * unfold open. rewrite <- open_preserves_size. omega. *)
+      (* * eapply closed_open. simpl. *)
+      eapply IHn with (H1 := H1); try eassumption || omega.
+      * unfold open. rewrite <- open_preserves_size. omega.
+      * eapply closed_open. simpl. eapply closed_upgrade_free.
+        eassumption.
+        all: omega || constructor; simpl; omega.
+      * eapply H2; assumption.
+  - inversion C. subst.
+    simpl in *.
+    assert (tsize_flat T1 < n) by omega.
+    rewrite val_type_unfold.
+    match_case_analysis; ev; repeat split_conj; simpl.
+    + eapply closed_upgrade_freef; eassumption || omega.
+    + intros.
+      eapply IHn with (H1 := H1); try eassumption || omega.
+      * unfold open. rewrite <- open_preserves_size. omega.
+      * eapply closed_open. simpl. eapply closed_upgrade_free.
+        eassumption.
+        all: omega || constructor; simpl; omega.
+      * eapply H2; assumption.
+    + eapply closed_upgrade_freef. eassumption. omega.
+
+    + intros.
+      (* eapply IHn with (H1 := H1). *)
+      (* * unfold open. rewrite <- open_preserves_size. omega. *)
+      (* * eapply closed_open. simpl. *)
+      eapply IHn with (H1 := H1); try eassumption || omega.
+      * unfold open. rewrite <- open_preserves_size. omega.
+      * eapply closed_open. simpl. eapply closed_upgrade_free.
+        eassumption.
+        all: omega || constructor; simpl; omega.
+      * eapply H2; assumption.
+    (* assert (closed 1 (length G1) (length H1) T1 /\ *)
+    (*     (exists jj : forall x : nat, vset x, *)
+    (*        jj k = df k /\ *)
+    (*        (forall n0 : nat, *)
+    (*         val_type H1 (jj :: G1) (open (varH (length G1)) T1) n0 (jj n0) vf))). destruct vf; assumption. clear V. ev. *)
+    (* assert (closed 1 (length G1) (length (vx :: H1)) T1 /\ *)
+    (* (exists jj : forall x0 : nat, vset x0, *)
+    (*    jj k = df k /\ *)
+    (*    (forall n0 : nat, *)
+    (*     val_type (vx :: H1) (jj :: G1) (open (varH (length G1)) T1) n0 *)
+    (*       (jj n0) vf))) as Goal. *)
+    (* split. simpl. eapply closed_upgrade_freef. eassumption. omega. *)
+    (* exists x. split. assumption. intros. specialize (H2 n0). eapply IHn with (H1 := H1). *)
+    (* unfold open. rewrite <- open_preserves_size. omega. *)
+    (* eapply closed_open. simpl. eapply closed_upgrade_free. eassumption. omega. *)
+    (* constructor. simpl. omega. *)
+    (* assumption. *)
+    (* destruct vf; apply Goal. *)
+
+  (* - inversion C. subst. rewrite val_type_unfold. *)
+  (*   assert (closed 1 (length G1) (length (vx :: H1)) T1 /\ *)
+  (*       (exists jj : forall x : nat, vset x, *)
+  (*          jj k = df k /\ *)
+  (*          (forall n0 : nat, *)
+  (*           val_type (vx :: H1) (jj :: G1) (open (varH (length G1)) T1) n0 *)
+  (*             (jj n0) vf))). destruct vf; assumption. clear V. ev. *)
+  (*   assert (closed 1 (length G1) (length H1) T1 /\ *)
+  (*   (exists jj : forall x0 : nat, vset x0, *)
+  (*      jj k = df k /\ *)
+  (*      (forall n0 : nat, *)
+  (*       val_type H1 (jj :: G1) (open (varH (length G1)) T1) n0 (jj n0) vf))) as Goal. *)
+  (*   split. assumption. exists x. split. assumption. intros. specialize (H2 n0). *)
+  (*   apply unvv. eapply IHn with (H1 := H1). unfold open. rewrite <- open_preserves_size. *)
+  (*   simpl in S. omega. eapply closed_open. simpl. eapply closed_upgrade_free. eassumption. omega. *)
+  (*   constructor. simpl. omega. apply vv. eassumption. *)
+  (*   destruct vf; apply Goal. *)
+
+  - inversion C. subst. simpl in *. rewrite val_type_unfold.
+    destruct vf. ev.
+    split. eapply IHn with (H1 := H1); try eassumption; try omega.
+    eapply IHn with (H1 := H1); try eassumption; try omega.
+    ev.
+    split. eapply IHn with (H1 := H1); try eassumption; try omega.
+    eapply IHn with (H1 := H1); try eassumption; try omega.
+  - inversion C. subst. simpl in *. rewrite val_type_unfold.
+    destruct vf. ev.
+    split. eapply IHn with (H1 := H1); try eassumption; try omega.
+    eapply IHn with (H1 := H1); try eassumption; try omega.
+    ev.
+    split. eapply IHn with (H1 := H1); try eassumption; try omega.
+    eapply IHn with (H1 := H1); try eassumption; try omega.
+Qed.
  
 
 (* (* used in wf_env_extend and in main theorem *) *)
-(* Lemma valtp_extend: forall vx vf df k G1 H1 T1, *)
-(*   val_type H1 G1 T1 k (df k) vf -> *)
-(*   vtp (vx::H1) G1 T1 k (df k) vf.  *)
+Lemma valtp_extend: forall vx vf k G1 H1 T1,
+  vtp H1 G1 T1 k  vf ->
+  vtp (vx::H1) G1 T1 k vf.
+Proof.
+  intros. eapply valtp_extend_aux with (H1 := H1) (n := tsize_flat T1 + 1).
+  - omega.
+  - apply valtp_closed in H. assumption.
+  - assumption.
+Qed.
+
+(* used in wf_env_extend *)
+Lemma valtp_shrink: forall vx vf k G1 H1 T1,
+  vtp (vx::H1) G1 T1 k vf ->
+  closed 0 (length G1) (length H1) T1 ->
+  vtp H1 G1 T1 k vf.
+Proof.
+  intros. eapply valtp_extend_aux. eauto. simpl. assumption.
+  eassumption.
+Qed.
+
+Lemma valtp_shrinkM: forall vx vf k H1 GH T1,
+  vtp (vx::H1) GH T1 k  vf ->
+  closed 0 (length GH) (length H1) T1 ->
+  vtp H1 GH T1 k vf.
+Proof.
+  intros. eapply valtp_extend_aux. eauto. simpl. assumption.
+  eassumption.
+Qed.
+
+Lemma indexr_hit_high: forall (X:Type) x (jj : X) l1 l2 vf,
+  indexr x (l1 ++ l2) = Some vf -> (length l2) <= x ->
+  indexr (x + 1) (l1 ++ jj :: l2) = Some vf.
+Proof. intros. induction l1. simpl in *. apply indexr_max in H. omega.
+  simpl in *. destruct (beq_nat x (length (l1 ++ l2))) eqn : A.
+  rewrite beq_nat_true_iff in A. assert (x + 1 = length (l1 ++ l2) + 1).
+  omega. rewrite app_length in *. assert(x + 1 = length (l1) + S (length l2)).
+  omega. simpl in *. rewrite <- beq_nat_true_iff in H2. rewrite H2. assumption.
+  rewrite beq_nat_false_iff in A. assert (x + 1 <> length (l1 ++ l2) + 1).
+  omega. rewrite app_length in *. assert(x + 1 <> length (l1) + S (length l2)). omega.
+  rewrite <- beq_nat_false_iff in H2. simpl. rewrite H2. apply IHl1. assumption.
+Qed.
+
+Lemma indexr_hit_low: forall (X:Type) x (jj : X) l1 l2 vf,
+  indexr x (l1 ++ l2) = Some vf -> x < (length l2) ->
+  indexr (x) (l1 ++ jj :: l2) = Some vf.
+Proof. intros. apply indexr_has in H0. ev. assert (indexr x (l1 ++ l2) = Some x0).
+  apply indexr_extend_mult. assumption. rewrite H1 in H. inversion H. subst.
+  assert (indexr x (jj :: l2) = Some vf). apply indexr_extend. assumption.
+  apply indexr_extend_mult. eassumption.
+Qed.
+
+Lemma splice_preserves_size: forall T j,
+  tsize_flat T = tsize_flat (splice j T).
+Proof.
+  intros. induction T; simpl; try rewrite IHT1; try rewrite IHT2; try reflexivity.
+  destruct v; simpl; try reflexivity. destruct (le_lt_dec j i); simpl; try reflexivity.
+  rewrite IHT. reflexivity.
+Qed.
+
+Lemma open_permute : forall T V0 V1 i j a b c d,
+  closed 0 a b (TSel V0) -> closed 0 c d (TSel V1) -> i <> j ->
+  open_rec i V0 (open_rec j V1 T) = open_rec j V1 (open_rec i V0 T).
+Proof. intros. generalize dependent i. generalize dependent j.
+  induction T; intros.
+  simpl. reflexivity.
+  simpl. reflexivity.
+  simpl. specialize (IHT1 _ _ H1). rewrite IHT1. assert ((S i) <> (S j)) by omega.
+  specialize (IHT2 _ _ H2). rewrite IHT2. reflexivity.
+  destruct v. simpl. reflexivity. simpl. reflexivity.
+  (* varB *)
+  destruct (beq_nat i i0) eqn : A. rewrite beq_nat_true_iff in A. subst.
+  assert ((open_rec j V1 (TSel (varB i0)) = (TSel (varB i0)))). simpl.
+  assert (beq_nat j i0 = false). rewrite beq_nat_false_iff. omega. rewrite H2. reflexivity.
+  rewrite H2. simpl. assert (beq_nat i0 i0 = true). erewrite beq_nat_refl. eauto. rewrite H3.
+  eapply closed_no_open. eapply closed_upgrade. eauto. omega.
+  destruct (beq_nat j i0) eqn : B. rewrite beq_nat_true_iff in B. subst.
+  simpl. assert (beq_nat i0 i0 = true). erewrite beq_nat_refl. eauto. rewrite H2.
+  assert (beq_nat i i0 = false). rewrite beq_nat_false_iff. omega. rewrite H3.
+  assert (TSel (V1) = open_rec i V0 (TSel V1)). eapply closed_no_open. eapply closed_upgrade.
+  eapply H0. omega. rewrite <- H4. simpl. rewrite H2. reflexivity.
+  assert ((open_rec j V1 (TSel (varB i0))) = TSel (varB i0)). simpl. rewrite B. reflexivity.
+  rewrite H2. assert (open_rec i V0 (TSel (varB i0)) = (TSel (varB i0))). simpl.
+  rewrite A. reflexivity. rewrite H3. simpl. rewrite B. reflexivity.
+
+  simpl. specialize (IHT1 _ _ H1). rewrite IHT1.
+  specialize (IHT2 _ _ H1). rewrite IHT2. reflexivity.
+  simpl. rewrite IHT. reflexivity. omega.
+  simpl. rewrite IHT1. rewrite IHT2. reflexivity. omega. omega.
+Qed.
+
+Lemma closed_open2: forall i j k V T i1, closed i j k T -> closed i j k (TSel V) ->
+  closed i j k (open_rec i1 V T).
+Proof.
+  intros. generalize dependent i. revert i1.
+  induction T; intros; inversion H;
+  try econstructor;
+  try eapply IHT1; eauto; try eapply IHT2; eauto; try eapply IHT; eauto.
+  eapply closed_upgrade. eauto. eauto.
+  - Case "TVarB". simpl.
+    case_eq (beq_nat i1 x); intros E. eauto.
+    econstructor. eapply beq_nat_false_iff in E. omega.
+  - eapply closed_upgrade. eassumption. omega.
+Qed.
+
+
+Lemma splice_retreat4: forall T i j k m V' V ,
+  closed i (j + 1) k (open_rec m V' (splice 0 T)) ->
+  (closed i j k (TSel V) -> closed i (j) k (open_rec m V T)).
+Proof. induction T; intros; try destruct v; simpl in *.
+  constructor.
+  constructor.
+  inversion H; subst.
+  specialize (IHT1 _ _ _ _ _ _ H6 H0). assert (closed (S i) (j) k (TSel V)).
+  eapply closed_upgrade. eapply H0. omega.
+  specialize (IHT2 _ _ _ _ _ _ H7 H1). constructor. assumption. assumption.
+  inversion H. subst. constructor. omega.
+  inversion H. subst. constructor. omega.
+  destruct (beq_nat m i0) eqn : A. assumption.
+    inversion H. subst. constructor. omega.
+  inversion H. subst. constructor. eapply IHT1. eassumption. assumption.
+  eapply IHT2. eassumption. assumption.
+  constructor. inversion H. subst.  eapply IHT; try eassumption. eapply closed_upgrade. eassumption. omega.
+  inversion H. subst. constructor.  eapply IHT1; try eassumption.
+  eapply IHT2; try eassumption.
+Qed.
+
+Lemma splice_retreat5: forall T i j k m V' V ,
+  closed i (j + 1) k (TSel V') -> closed i (j) k (open_rec m V T) ->
+  closed i (j + 1) k (open_rec m V' (splice 0 T)).
+Proof. induction T; intros; try destruct v; simpl in *.
+  constructor.
+  constructor.
+  inversion H0; subst.
+  specialize (IHT1 _ _ _ _ _ _ H H6). assert (closed (S i) (j + 1) k (TSel V')).
+  eapply closed_upgrade. eapply H. omega.
+  specialize (IHT2 _ _ _ _ _ _ H1 H7). constructor. assumption. assumption.
+  inversion H0. subst. constructor. omega.
+  inversion H0. subst. constructor. omega.
+  destruct (beq_nat m i0) eqn : A. assumption.
+    inversion H0. subst. constructor. omega.
+  inversion H0. subst. constructor. eapply IHT1. eassumption. eassumption.
+  eapply IHT2. eassumption. eassumption.
+  inversion H0. subst. constructor. eapply IHT; try eassumption. eapply closed_upgrade. eassumption. omega.
+  inversion H0. subst. constructor. eapply IHT1; try eassumption. eapply IHT2; try eassumption.
+
+Qed.
+
+
+
+Lemma splice_open_permute0: forall x0 T2 n j,
+(open_rec j (varH (n + x0 + 1 )) (splice (x0) T2)) =
+(splice (x0) (open_rec j (varH (n + x0)) T2)).
+Proof.
+  intros x0 T. induction T; intros; simpl; eauto;
+  try rewrite IHT1; try rewrite IHT2; try rewrite IHT; eauto;
+  destruct v; eauto.
+
+  case_eq (le_lt_dec (x0) i); intros E LE; simpl; eauto.
+  rewrite LE. eauto.
+  rewrite LE. eauto.
+  case_eq (beq_nat j i); intros E; simpl; eauto.
+  case_eq (le_lt_dec (x0) (n + x0)); intros EL LE.
+  rewrite E. eauto. omega.
+  rewrite E. eauto.
+Qed.
+
+Lemma indexr_extend_end: forall {X : Type} (jj : X) l x,
+  indexr (x + 1) (l ++ [jj]) = indexr x l.
+Proof. intros. induction l. simpl. assert (beq_nat (x + 1) 0 = false).
+  rewrite beq_nat_false_iff. omega. rewrite H. reflexivity.
+  simpl. destruct (beq_nat (x) (length (l))) eqn : A.
+  rewrite beq_nat_true_iff in A. assert (x + 1 = length (l ++ [jj])). rewrite app_length. simpl. omega.
+  rewrite <- beq_nat_true_iff in H. rewrite H. reflexivity.
+  rewrite beq_nat_false_iff in A. assert (x +1 <> length (l ++ [jj])). rewrite app_length. simpl. omega.
+  rewrite <- beq_nat_false_iff in H. rewrite H. assumption.
+Qed.
+
+Lemma indexr_hit01: forall {X : Type} GH (jj : X),
+      indexr 0 (GH ++ [jj]) = Some (jj).
+Proof.
+  intros X GH. induction GH.
+  - intros. simpl. eauto.
+  - intros. simpl. destruct (length (GH ++ [jj])) eqn : A.
+    rewrite app_length in *. simpl in *. omega.
+    apply IHGH.
+Qed.
   
-(* Proof. *)
-(*   intros. eapply valtp_extend_aux with (H1 := H1). eauto. simpl. *)
-(*   apply valtp_closed in H. simpl in *. assumption. apply vv in H. assumption. *)
-(* Qed. *)
-
-(* (* used in wf_env_extend *) *)
-(* Lemma valtp_shrink: forall vx vf df k G1 H1 T1, *)
-(*   val_type (vx::H1) G1 T1 k (df k) vf -> *)
-(*   closed 0 (length G1) (length H1) T1 ->                      *)
-(*   vtp H1 G1 T1 k (df k) vf. *)
-(* Proof. *)
-(*   intros. apply vv in H. eapply valtp_extend_aux. eauto. simpl. assumption. *)
-(*   eassumption. *)
-(* Qed. *)
-
-(* Lemma valtp_shrinkM: forall vx vf df k H1 GH T1, *)
-(*   val_type (vx::H1) GH T1 k (df k) vf -> *)
-(*   closed 0 (length GH) (length H1) T1 ->                      *)
-(*   vtp H1 GH T1 k (df k) vf. *)
-(* Proof. *)
-(*   intros. apply vv in H. eapply valtp_extend_aux. eauto. simpl. assumption. *)
-(*   eassumption. *)
-(* Qed. *)
-
-(* Lemma indexr_hit_high: forall (X:Type) x (jj : X) l1 l2 vf, *)
-(*   indexr x (l1 ++ l2) = Some vf -> (length l2) <= x -> *)
-(*   indexr (x + 1) (l1 ++ jj :: l2) = Some vf. *)
-(* Proof. intros. induction l1. simpl in *. apply indexr_max in H. omega. *)
-(*   simpl in *. destruct (beq_nat x (length (l1 ++ l2))) eqn : A. *)
-(*   rewrite beq_nat_true_iff in A. assert (x + 1 = length (l1 ++ l2) + 1). *)
-(*   omega. rewrite app_length in *. assert(x + 1 = length (l1) + S (length l2)). *)
-(*   omega. simpl in *. rewrite <- beq_nat_true_iff in H2. rewrite H2. assumption. *)
-(*   rewrite beq_nat_false_iff in A. assert (x + 1 <> length (l1 ++ l2) + 1). *)
-(*   omega. rewrite app_length in *. assert(x + 1 <> length (l1) + S (length l2)). omega. *)
-(*   rewrite <- beq_nat_false_iff in H2. simpl. rewrite H2. apply IHl1. assumption. *)
-(* Qed. *)
-
-(* Lemma indexr_hit_low: forall (X:Type) x (jj : X) l1 l2 vf, *)
-(*   indexr x (l1 ++ l2) = Some vf -> x < (length l2) -> *)
-(*   indexr (x) (l1 ++ jj :: l2) = Some vf. *)
-(* Proof. intros. apply indexr_has in H0. ev. assert (indexr x (l1 ++ l2) = Some x0). *)
-(*   apply indexr_extend_mult. assumption. rewrite H1 in H. inversion H. subst. *)
-(*   assert (indexr x (jj :: l2) = Some vf). apply indexr_extend. assumption. *)
-(*   apply indexr_extend_mult. eassumption. *)
-(* Qed. *)
-
-(* Lemma splice_preserves_size: forall T j, *)
-(*   tsize_flat T = tsize_flat (splice j T). *)
-(* Proof. *)
-(*   intros. induction T; simpl; try rewrite IHT1; try rewrite IHT2; try reflexivity. *)
-(*   destruct v; simpl; try reflexivity. destruct (le_lt_dec j i); simpl; try reflexivity. *)
-(*   rewrite IHT. reflexivity. *)
-(* Qed. *)
-
-(* Lemma open_permute : forall T V0 V1 i j a b c d, *)
-(*   closed 0 a b (TSel V0) -> closed 0 c d (TSel V1) -> i <> j -> *)
-(*   open_rec i V0 (open_rec j V1 T) = open_rec j V1 (open_rec i V0 T). *)
-(* Proof. intros. generalize dependent i. generalize dependent j. *)
-(*   induction T; intros. *)
-(*   simpl. reflexivity. *)
-(*   simpl. reflexivity. *)
-(*   simpl. specialize (IHT1 _ _ H1). rewrite IHT1. assert ((S i) <> (S j)) by omega. *)
-(*   specialize (IHT2 _ _ H2). rewrite IHT2. reflexivity. *)
-(*   destruct v. simpl. reflexivity. simpl. reflexivity. *)
-(*   (* varB *) *)
-(*   destruct (beq_nat i i0) eqn : A. rewrite beq_nat_true_iff in A. subst. *)
-(*   assert ((open_rec j V1 (TSel (varB i0)) = (TSel (varB i0)))). simpl.  *)
-(*   assert (beq_nat j i0 = false). rewrite beq_nat_false_iff. omega. rewrite H2. reflexivity. *)
-(*   rewrite H2. simpl. assert (beq_nat i0 i0 = true). erewrite beq_nat_refl. eauto. rewrite H3.  *)
-(*   eapply closed_no_open. eapply closed_upgrade. eauto. omega. *)
-(*   destruct (beq_nat j i0) eqn : B. rewrite beq_nat_true_iff in B. subst. *)
-(*   simpl. assert (beq_nat i0 i0 = true). erewrite beq_nat_refl. eauto. rewrite H2. *)
-(*   assert (beq_nat i i0 = false). rewrite beq_nat_false_iff. omega. rewrite H3. *)
-(*   assert (TSel (V1) = open_rec i V0 (TSel V1)). eapply closed_no_open. eapply closed_upgrade. *)
-(*   eapply H0. omega. rewrite <- H4. simpl. rewrite H2. reflexivity. *)
-(*   assert ((open_rec j V1 (TSel (varB i0))) = TSel (varB i0)). simpl. rewrite B. reflexivity. *)
-(*   rewrite H2. assert (open_rec i V0 (TSel (varB i0)) = (TSel (varB i0))). simpl. *)
-(*   rewrite A. reflexivity. rewrite H3. simpl. rewrite B. reflexivity. *)
-
-(*   simpl. specialize (IHT1 _ _ H1). rewrite IHT1. *)
-(*   specialize (IHT2 _ _ H1). rewrite IHT2. reflexivity. *)
-(*   simpl. rewrite IHT. reflexivity. omega. *)
-(*   simpl. rewrite IHT1. rewrite IHT2. reflexivity. omega. omega. *)
-(* Qed. *)
-
-(* Lemma closed_open2: forall i j k V T i1, closed i j k T -> closed i j k (TSel V) -> *)
-(*   closed i j k (open_rec i1 V T). *)
-(* Proof. *)
-(*   intros. generalize dependent i. revert i1. *)
-(*   induction T; intros; inversion H; *)
-(*   try econstructor; *)
-(*   try eapply IHT1; eauto; try eapply IHT2; eauto; try eapply IHT; eauto. *)
-(*   eapply closed_upgrade. eauto. eauto. *)
-(*   - Case "TVarB". simpl. *)
-(*     case_eq (beq_nat i1 x); intros E. eauto. *)
-(*     econstructor. eapply beq_nat_false_iff in E. omega. *)
-(*   - eapply closed_upgrade. eassumption. omega. *)
-(* Qed. *)
 
 
-(* Lemma splice_retreat4: forall T i j k m V' V , *)
-(*   closed i (j + 1) k (open_rec m V' (splice 0 T)) -> *)
-(*   (closed i j k (TSel V) -> closed i (j) k (open_rec m V T)). *)
-(* Proof. induction T; intros; try destruct v; simpl in *. *)
-(*   constructor. *)
-(*   constructor. *)
-(*   inversion H; subst.  *)
-(*   specialize (IHT1 _ _ _ _ _ _ H6 H0). assert (closed (S i) (j) k (TSel V)). *)
-(*   eapply closed_upgrade. eapply H0. omega. *)
-(*   specialize (IHT2 _ _ _ _ _ _ H7 H1). constructor. assumption. assumption.  *)
-(*   inversion H. subst. constructor. omega. *)
-(*   inversion H. subst. constructor. omega. *)
-(*   destruct (beq_nat m i0) eqn : A. assumption.  *)
-(*     inversion H. subst. constructor. omega. *)
-(*   inversion H. subst. constructor. eapply IHT1. eassumption. assumption. *)
-(*   eapply IHT2. eassumption. assumption. *)
-(*   constructor. inversion H. subst.  eapply IHT; try eassumption. eapply closed_upgrade. eassumption. omega. *)
-(*   inversion H. subst. constructor.  eapply IHT1; try eassumption.  *)
-(*   eapply IHT2; try eassumption. *)
-(* Qed. *)
-
-(* Lemma splice_retreat5: forall T i j k m V' V , *)
-(*   closed i (j + 1) k (TSel V') -> closed i (j) k (open_rec m V T) -> *)
-(*   closed i (j + 1) k (open_rec m V' (splice 0 T)). *)
-(* Proof. induction T; intros; try destruct v; simpl in *. *)
-(*   constructor. *)
-(*   constructor. *)
-(*   inversion H0; subst. *)
-(*   specialize (IHT1 _ _ _ _ _ _ H H6). assert (closed (S i) (j + 1) k (TSel V')). *)
-(*   eapply closed_upgrade. eapply H. omega. *)
-(*   specialize (IHT2 _ _ _ _ _ _ H1 H7). constructor. assumption. assumption.  *)
-(*   inversion H0. subst. constructor. omega. *)
-(*   inversion H0. subst. constructor. omega. *)
-(*   destruct (beq_nat m i0) eqn : A. assumption.  *)
-(*     inversion H0. subst. constructor. omega. *)
-(*   inversion H0. subst. constructor. eapply IHT1. eassumption. eassumption. *)
-(*   eapply IHT2. eassumption. eassumption. *)
-(*   inversion H0. subst. constructor. eapply IHT; try eassumption. eapply closed_upgrade. eassumption. omega. *)
-(*   inversion H0. subst. constructor. eapply IHT1; try eassumption. eapply IHT2; try eassumption. *)
-
-(* Qed. *)
-
-
-
-(* Lemma splice_open_permute0: forall x0 T2 n j, *)
-(* (open_rec j (varH (n + x0 + 1 )) (splice (x0) T2)) = *)
-(* (splice (x0) (open_rec j (varH (n + x0)) T2)). *)
-(* Proof. *)
-(*   intros x0 T. induction T; intros; simpl; eauto; *)
-(*   try rewrite IHT1; try rewrite IHT2; try rewrite IHT; eauto; *)
-(*   destruct v; eauto. *)
-
-(*   case_eq (le_lt_dec (x0) i); intros E LE; simpl; eauto. *)
-(*   rewrite LE. eauto. *)
-(*   rewrite LE. eauto. *)
-(*   case_eq (beq_nat j i); intros E; simpl; eauto. *)
-(*   case_eq (le_lt_dec (x0) (n + x0)); intros EL LE. *)
-(*   rewrite E. eauto. omega. *)
-(*   rewrite E. eauto. *)
-(* Qed. *)
-
-(* Lemma indexr_extend_end: forall {X : Type} (jj : X) l x, *)
-(*   indexr (x + 1) (l ++ [jj]) = indexr x l. *)
-(* Proof. intros. induction l. simpl. assert (beq_nat (x + 1) 0 = false). *)
-(*   rewrite beq_nat_false_iff. omega. rewrite H. reflexivity. *)
-(*   simpl. destruct (beq_nat (x) (length (l))) eqn : A. *)
-(*   rewrite beq_nat_true_iff in A. assert (x + 1 = length (l ++ [jj])). rewrite app_length. simpl. omega. *)
-(*   rewrite <- beq_nat_true_iff in H. rewrite H. reflexivity. *)
-(*   rewrite beq_nat_false_iff in A. assert (x +1 <> length (l ++ [jj])). rewrite app_length. simpl. omega. *)
-(*   rewrite <- beq_nat_false_iff in H. rewrite H. assumption. *)
-(* Qed. *)
-
-(* Lemma indexr_hit01: forall {X : Type} GH (jj : X), *)
-(*       indexr 0 (GH ++ [jj]) = Some (jj). *)
-(* Proof. *)
-(*   intros X GH. induction GH. *)
-(*   - intros. simpl. eauto. *)
-(*   - intros. simpl. destruct (length (GH ++ [jj])) eqn : A. *)
-(*     rewrite app_length in *. simpl in *. omega. *)
-(*     apply IHGH. *)
-(* Qed.   *)
-  
-
-
-(* Lemma valtp_splice_aux: forall n T vf H GH1 GH0 jj df k, *)
-(* tsize_flat T < n -> closed 0 (length (GH1 ++ GH0)) (length H) T -> *)
-(* (   *)
-(*   vtp H (GH1 ++ GH0) T k (df k) vf <->  *)
-(*   vtp H (GH1 ++ jj :: GH0) (splice (length GH0) T) k (df k) vf *)
-(* ). *)
-(* Proof. *)
-(*   induction n; intros ? ? ? ? ? ? ? ? Sz C. inversion Sz. *)
-(*   destruct T; split; intros V; apply unvv in V; simpl in *; rewrite val_type_unfold in V; *)
-(*     assert (length GH1 + S (length GH0) = S(length (GH1 ++ GH0))) as E; *)
-(*     try rewrite app_length; try omega. *)
-(*   - apply vv. rewrite val_type_unfold. destruct vf; apply V. *)
-(*   - apply vv. rewrite val_type_unfold. destruct vf; apply V. *)
-(*   - apply vv. rewrite val_type_unfold. destruct vf; apply V. *)
-(*   - apply vv. rewrite val_type_unfold. destruct vf; apply V. *)
-(*   - destruct vf; try solve by inversion.  *)
-(*     ev. apply vv. simpl. rewrite val_type_unfold.  *)
-(*     split. rewrite app_length. simpl. rewrite E. apply closed_splice. apply H0. *)
-(*     split. rewrite app_length. simpl. rewrite E. apply closed_splice. apply H1. *)
-(*     intros. assert (forall kx : nat, val_type H (GH1 ++ GH0) T1 kx (jj0 kx) vx). *)
-(*     intros. apply unvv. eapply IHn. simpl in Sz. omega. assumption. apply vv. apply H3.  *)
-(*     specialize (H2 _ _ H4).  *)
-(*     ev. exists x. exists x0. split. assumption. intros. specialize (H5 k0). *)
-(*     apply unvv. rewrite app_comm_cons. rewrite app_comm_cons in H5. *)
-(*     unfold open. rewrite app_length. replace (length (jj::GH0)) with (length GH0 + 1). rewrite plus_assoc. *)
-(*     rewrite splice_open_permute0. eapply IHn with (GH0 := GH0).  *)
-(*     rewrite <- open_preserves_size. simpl in Sz. omega. *)
-(*     eapply closed_open. simpl. eapply closed_upgrade_free. eassumption. omega. *)
-(*     constructor. simpl. rewrite app_length. omega. *)
-(*     apply vv. unfold open in *. rewrite app_length in *. assumption. *)
-(*     simpl. omega. *)
+Lemma valtp_splice_aux: forall n T vf H GH1 GH0 vl k,
+tsize_flat T < n -> closed 0 (length (GH1 ++ GH0)) (length H) T ->
+(
+  vtp H (GH1 ++ GH0) T k vf <->
+  vtp H (GH1 ++ vl :: GH0) (splice (length GH0) T) k vf
+).
+Proof.
+  induction n; intros * Sz C. inversion Sz.
+  destruct T; split; intros V; simpl in *; rewrite val_type_unfold in V;
+    assert (length GH1 + S (length GH0) = S (length (GH1 ++ GH0))) as E;
+    try rewrite app_length; try omega.
+  - rewrite val_type_unfold. destruct vf; apply V.
+  - rewrite val_type_unfold. destruct vf; apply V.
+  - rewrite val_type_unfold. destruct vf; apply V.
+  - rewrite val_type_unfold. destruct vf; apply V.
+  - destruct vf; try solve by inversion.
+    ev. simpl. rewrite val_type_unfold.
+    repeat split_conj.
+    + rewrite app_length. simpl. rewrite E. apply closed_splice. apply H0.
+    + rewrite app_length. simpl. rewrite E. apply closed_splice. apply H1.
+    + intros.
+      assert (tsize_flat T1 + tsize_flat T2 < n) by omega.
+      assert (vtp H (GH1 ++ GH0) T1 j vx).
+      * intros. eapply IHn; (omega || eassumption).
+      * specialize (H2 _ _ Hj H5).
+        ev. exists x. split. assumption.
+        rewrite app_comm_cons.
+        (* rewrite app_comm_cons in H5. *)
+        unfold open. rewrite app_length.
+        replace (length (vl::GH0)) with (length GH0 + 1) by (simpl; omega).
+        rewrite plus_assoc.
+        rewrite splice_open_permute0.
+        eapply IHn with (GH0 := GH0).
+        -- rewrite <- open_preserves_size. omega.
+        -- eapply closed_open. simpl. eapply closed_upgrade_free. eassumption. omega.
+           constructor. simpl. rewrite app_length. omega.
+        -- unfold open in *. rewrite app_length in *. assumption.
     
-(*   - destruct vf; try solve by inversion. simpl in V. *)
-(*     ev. apply vv. rewrite val_type_unfold. inversion C. subst. *)
-(*     split. assumption. split. assumption. intros. *)
-(*     assert (forall kx : nat, val_type H (GH1 ++ jj :: GH0) (splice (length GH0) T1) kx (jj0 kx) vx). *)
-(*     intros. specialize (H3 kx). apply unvv. eapply IHn with (GH0:= GH0). *)
-(*     simpl in Sz. omega. *)
-(*     assumption. *)
-(*     apply vv. assumption. *)
-(*     specialize (H2 _ _ H4). ev. exists x. exists x0. *)
-(*     split. assumption. intros. specialize (H5 k0). apply unvv. rewrite app_comm_cons. *)
-(*     eapply IHn with (GH0 := GH0). unfold open. rewrite <- open_preserves_size. simpl in Sz. omega. *)
-(*     apply closed_open. simpl. eapply closed_upgrade_free. eassumption. omega. *)
-(*     constructor. simpl. omega. *)
-(*     apply vv. rewrite app_length in H5. simpl in H5. replace ( S(length GH0)) with (length GH0 + 1) in H5. *)
-(*     rewrite plus_assoc in H5. unfold open in H5. rewrite splice_open_permute0 in H5. *)
-(*     rewrite app_length. unfold open. eassumption.  *)
-(*     simpl. omega. *)
+  - destruct vf; try solve by inversion. simpl in V.
+    ev. rewrite val_type_unfold. inversion C. subst.
+    split. assumption. split. assumption. intros.
+    assert (tsize_flat T1 + tsize_flat T2 < n) by omega.
+    assert (vtp H (GH1 ++ vl :: GH0) (splice (length GH0) T1) j vx) by
+        (eapply IHn with (GH0 := GH0); try (omega || eassumption)).
+   specialize (H2 _ _ Hj H5). ev. exists x.
+    split_conj; try assumption.
+    intros. rewrite app_comm_cons.
+    eapply IHn with (GH0 := GH0).
+    + unfold open. rewrite <- open_preserves_size. omega.
+    + apply closed_open. simpl. eapply closed_upgrade_free. eassumption. omega.
+      constructor. simpl. omega.
+    +
+      rewrite app_length in H6. simpl in H6.
+      replace (S (length GH0)) with (length GH0 + 1) in H6 by (simpl; omega).
+      rewrite plus_assoc in H6. unfold open in H6. rewrite splice_open_permute0 in H6.
+      rewrite app_length. unfold open. eassumption.
     
-(*   - apply vv. rewrite val_type_unfold. destruct vf. simpl in *. destruct v. *)
-(*     + assumption.  *)
-(*     + destruct (indexr i (GH1 ++ GH0)) eqn : B; try solve by inversion.  *)
-(*     destruct (le_lt_dec (length GH0) i) eqn : A.  *)
-(*     assert (indexr (i + 1) (GH1 ++ jj :: GH0) = Some v). apply indexr_hit_high. assumption. omega. *)
-(*     rewrite H0. apply V. assert (indexr (i) (GH1 ++ jj :: GH0) = Some v). apply indexr_hit_low. assumption. omega. *)
+  - rewrite val_type_unfold.
+    (* simpl in *. match_case_analysis. *)
+    destruct vf. simpl in *. destruct v.
+    (* + assumption. *)
+    + destruct (indexr i H) eqn : B; try solve by inversion.
+      match_case_analysis.
+      intros.
+      Admitted.
+
+(*     + destruct (indexr i (GH1 ++ GH0)) eqn : B; try solve by inversion. *)
+(*     destruct (le_lt_dec (length GH0) i) eqn : A. *)
+(*     assert (indexr (i + 1) (GH1 ++ vl :: GH0) = Some v). apply indexr_hit_high. assumption. omega. *)
+(*     rewrite H0. apply V. assert (indexr (i) (GH1 ++ vl :: GH0) = Some v). apply indexr_hit_low. assumption. omega. *)
 (*     rewrite H0. apply V. *)
 (*     + inversion V. *)
 (*     + simpl in *. destruct v; simpl; try apply V. *)
-(*     destruct (indexr i (GH1 ++ GH0)) eqn : B; try solve by inversion.  *)
-(*     destruct (le_lt_dec (length GH0) i) eqn : A.  *)
-(*     assert (indexr (i + 1) (GH1 ++ jj :: GH0) = Some v). apply indexr_hit_high. assumption. omega. *)
-(*     rewrite H0. apply V. assert (indexr (i) (GH1 ++ jj :: GH0) = Some v). apply indexr_hit_low. assumption. omega. *)
+(*     destruct (indexr i (GH1 ++ GH0)) eqn : B; try solve by inversion. *)
+(*     destruct (le_lt_dec (length GH0) i) eqn : A. *)
+(*     assert (indexr (i + 1) (GH1 ++ vl :: GH0) = Some v). apply indexr_hit_high. assumption. omega. *)
+(*     rewrite H0. apply V. assert (indexr (i) (GH1 ++ vl :: GH0) = Some v). apply indexr_hit_low. assumption. omega. *)
 (*     rewrite H0. apply V. *)
 
 (*   - apply vv. rewrite val_type_unfold. destruct vf; simpl in *. destruct v. *)
 (*     + assumption. *)
-(*     + destruct (le_lt_dec (length GH0) i) eqn : A. inversion C. subst.   *)
-(*     eapply indexr_has in H4. ev. assert (indexr (i + 1)(GH1 ++ jj:: GH0) = Some x). apply indexr_hit_high; assumption.  *)
-(*     rewrite H0. rewrite H1 in V. assumption.  *)
+(*     + destruct (le_lt_dec (length GH0) i) eqn : A. inversion C. subst. *)
+(*     eapply indexr_has in H4. ev. assert (indexr (i + 1)(GH1 ++ vl:: GH0) = Some x). apply indexr_hit_high; assumption. *)
+(*     rewrite H0. rewrite H1 in V. assumption. *)
 (*     assert (i < length GH0) as H4 by omega. eapply indexr_has in H4. ev. assert (indexr (i)(GH1 ++ GH0) = Some x). *)
-(*     apply indexr_extend_mult. assumption. assert (indexr i (GH1 ++ jj :: GH0) = Some x). apply indexr_hit_low; assumption.  *)
+(*     apply indexr_extend_mult. assumption. assert (indexr i (GH1 ++ vl :: GH0) = Some x). apply indexr_hit_low; assumption. *)
 (*     rewrite H1. rewrite H2 in V. assumption. *)
 (*     + inversion V. *)
 (*     + destruct v; try solve by inversion; try assumption. *)
-(*     destruct (le_lt_dec (length GH0) i) eqn : A. inversion C. subst.  *)
-(*     eapply indexr_has in H4. ev. assert (indexr (i + 1)(GH1 ++ jj:: GH0) = Some x). apply indexr_hit_high; assumption.  *)
-(*     rewrite H0. rewrite H1 in V. assumption.  *)
+(*     destruct (le_lt_dec (length GH0) i) eqn : A. inversion C. subst. *)
+(*     eapply indexr_has in H4. ev. assert (indexr (i + 1)(GH1 ++ vl:: GH0) = Some x). apply indexr_hit_high; assumption. *)
+(*     rewrite H0. rewrite H1 in V. assumption. *)
 (*     assert (i < length GH0) as H4 by omega. eapply indexr_has in H4. ev. assert (indexr (i)(GH1 ++ GH0) = Some x). *)
-(*     apply indexr_extend_mult. assumption. assert (indexr i (GH1 ++ jj :: GH0) = Some x). apply indexr_hit_low; assumption.  *)
+(*     apply indexr_extend_mult. assumption. assert (indexr i (GH1 ++ vl :: GH0) = Some x). apply indexr_hit_low; assumption. *)
 (*     rewrite H1. rewrite H2 in V. assumption. *)
 
 (*   - inversion C. subst. apply vv. rewrite val_type_unfold. destruct vf; try solve by inversion. *)
-(*     simpl in *. ev.  *)
+(*     simpl in *. ev. *)
 (*     split. rewrite app_length. simpl. rewrite E. eapply closed_splice. assumption. *)
 (*     split. rewrite app_length. simpl. rewrite E. eapply closed_splice. assumption. *)
 (*     destruct k. auto. intros. specialize (H2 dy vy). ev. split. intros. apply H2. *)
@@ -1321,7 +1413,7 @@ Definition R_env venv genv tenv :=
 (*     intros. specialize (H3 H4). apply unvv. eapply IHn with (GH0 := GH0). simpl in Sz. omega. *)
 (*     assumption. apply vv. assumption. *)
 
-(*   - inversion C. subst. apply vv. rewrite val_type_unfold. destruct vf; try solve by inversion.  *)
+(*   - inversion C. subst. apply vv. rewrite val_type_unfold. destruct vf; try solve by inversion. *)
 (*     simpl in *. ev. split. assumption. split. assumption. destruct k. auto. *)
 (*     intros. specialize (H2 dy vy). ev. split. intros. *)
 (*     apply H2. apply unvv. eapply IHn with (GH0 := GH0). simpl in Sz. omega. *)
@@ -1331,23 +1423,23 @@ Definition R_env venv genv tenv :=
 
 (*   - inversion C. subst. simpl in *. apply vv. rewrite val_type_unfold. *)
 (*     assert (closed 1 (length (GH1 ++ GH0)) (length H) T /\ *)
-(*         (exists jj0 : forall x : nat, vset x, *)
-(*            jj0 k = df k /\ *)
+(*         (exists vl0 : forall x : nat, vset x, *)
+(*            vl0 k = df k /\ *)
 (*            (forall n0 : nat, *)
-(*             val_type H (jj0 :: GH1 ++ GH0) *)
-(*               (open (varH (length (GH1 ++ GH0))) T) n0 (jj0 n0) vf))). *)
+(*             val_type H (vl0 :: GH1 ++ GH0) *)
+(*               (open (varH (length (GH1 ++ GH0))) T) n0 (vl0 n0) vf))). *)
 (*               destruct vf; assumption. clear V. ev. *)
-(*     assert (closed 1 (length (GH1 ++ jj :: GH0)) (length H) (splice (length GH0) T) /\ *)
-(*     (exists jj0 : forall x : nat, vset x, *)
-(*        jj0 k = df k /\ *)
+(*     assert (closed 1 (length (GH1 ++ vl :: GH0)) (length H) (splice (length GH0) T) /\ *)
+(*     (exists vl0 : forall x : nat, vset x, *)
+(*        vl0 k = df k /\ *)
 (*        (forall n0 : nat, *)
-(*         val_type H (jj0 :: GH1 ++ jj :: GH0) *)
-(*           (open (varH (length (GH1 ++ jj :: GH0))) (splice (length GH0) T)) *)
-(*           n0 (jj0 n0) vf))) as Goal. *)
+(*         val_type H (vl0 :: GH1 ++ vl :: GH0) *)
+(*           (open (varH (length (GH1 ++ vl :: GH0))) (splice (length GH0) T)) *)
+(*           n0 (vl0 n0) vf))) as Goal. *)
 (*     split. rewrite app_length. simpl. rewrite <- plus_n_Sm. eapply closed_splice. *)
 (*     rewrite <- app_length. assumption. *)
 (*     exists x. split. assumption. *)
-(*     intros. specialize (H2 n0). apply unvv. rewrite app_length. replace (length (jj::GH0)) with (length GH0 + 1). *)
+(*     intros. specialize (H2 n0). apply unvv. rewrite app_length. replace (length (vl::GH0)) with (length GH0 + 1). *)
 (*     rewrite plus_assoc. unfold open. rewrite splice_open_permute0. rewrite app_comm_cons. eapply IHn with (GH0 := GH0). *)
 (*     rewrite <- open_preserves_size. simpl in Sz. omega. *)
 (*     eapply closed_open. simpl. eapply closed_upgrade_free. eassumption. omega. *)
@@ -1357,37 +1449,37 @@ Definition R_env venv genv tenv :=
 (*     destruct vf; apply Goal. *)
 
 (*   - inversion C. subst. simpl in *. apply vv. rewrite val_type_unfold. *)
-(*     assert (closed 1 (length (GH1 ++ jj :: GH0)) (length H) *)
+(*     assert (closed 1 (length (GH1 ++ vl :: GH0)) (length H) *)
 (*           (splice (length GH0) T) /\ *)
-(*         (exists jj0 : forall x : nat, vset x, *)
-(*            jj0 k = df k /\ *)
+(*         (exists vl0 : forall x : nat, vset x, *)
+(*            vl0 k = df k /\ *)
 (*            (forall n0 : nat, *)
-(*             val_type H (jj0 :: GH1 ++ jj :: GH0) *)
-(*               (open (varH (length (GH1 ++ jj :: GH0))) *)
-(*                  (splice (length GH0) T)) n0 (jj0 n0) vf))). destruct vf; assumption. clear V. ev. *)
+(*             val_type H (vl0 :: GH1 ++ vl :: GH0) *)
+(*               (open (varH (length (GH1 ++ vl :: GH0))) *)
+(*                  (splice (length GH0) T)) n0 (vl0 n0) vf))). destruct vf; assumption. clear V. ev. *)
 (*     assert (closed 1 (length (GH1 ++ GH0)) (length H) T /\ *)
-(*     (exists jj0 : forall x0 : nat, vset x0, *)
-(*        jj0 k = df k /\ *)
+(*     (exists vl0 : forall x0 : nat, vset x0, *)
+(*        vl0 k = df k /\ *)
 (*        (forall n0 : nat, *)
-(*         val_type H (jj0 :: GH1 ++ GH0) (open (varH (length (GH1 ++ GH0))) T) *)
-(*           n0 (jj0 n0) vf))) as Goal. *)
+(*         val_type H (vl0 :: GH1 ++ GH0) (open (varH (length (GH1 ++ GH0))) T) *)
+(*           n0 (vl0 n0) vf))) as Goal. *)
 (*     split. assumption. exists x. split. assumption. *)
 (*     intros. specialize (H2 n0). apply unvv. rewrite app_comm_cons. eapply IHn with (GH0 := GH0). *)
 (*     unfold open. rewrite <- open_preserves_size. simpl in Sz. omega. *)
 (*     apply closed_open. simpl. eapply closed_upgrade_free. eassumption. omega. *)
 (*     constructor. simpl. omega. *)
-(*     rewrite app_length in H2. replace (length (jj :: GH0)) with (length GH0 + 1) in H2. *)
+(*     rewrite app_length in H2. replace (length (vl :: GH0)) with (length GH0 + 1) in H2. *)
 (*     unfold open in H2. rewrite plus_assoc in H2. rewrite splice_open_permute0 in H2. *)
 (*     rewrite app_length. unfold open. apply vv. eassumption. *)
 (*     simpl. omega. *)
 (*     destruct vf; apply Goal. *)
 
-(*   - inversion C. subst. simpl in *. apply vv. rewrite val_type_unfold. destruct vf; ev.  *)
+(*   - inversion C. subst. simpl in *. apply vv. rewrite val_type_unfold. destruct vf; ev. *)
 (*     split. apply unvv. apply vv in H0. eapply IHn with (GH0 := GH0); try eassumption; try omega. *)
 (*     apply unvv. apply vv in H1. eapply IHn with (GH0 := GH0); try eassumption; try omega. *)
 (*     split. apply unvv. apply vv in H0. eapply IHn with (GH0 := GH0); try eassumption; try omega. *)
 (*     apply unvv. apply vv in H1. eapply IHn with (GH0 := GH0); try eassumption; try omega. *)
-(*   - inversion C. subst. simpl in *. apply vv. rewrite val_type_unfold. destruct vf; ev.  *)
+(*   - inversion C. subst. simpl in *. apply vv. rewrite val_type_unfold. destruct vf; ev. *)
 (*     split. apply unvv. apply vv in H0. eapply IHn with (GH0 := GH0); try eassumption; try omega. *)
 (*     apply unvv. apply vv in H1. eapply IHn with (GH0 := GH0); try eassumption; try omega. *)
 (*     split. apply unvv. apply vv in H0. eapply IHn with (GH0 := GH0); try eassumption; try omega. *)
@@ -1396,52 +1488,53 @@ Definition R_env venv genv tenv :=
 (* Qed. *)
 
 
-(* (* used in valtp_widen *) *)
-(* Lemma valtp_extendH: forall vf df k H1 GH T1 jj, *)
-(*   val_type H1 GH T1 k (df k) vf ->  *)
-(*   vtp H1 (jj::GH) T1 k (df k) vf. *)
-(* Proof. *)
-(*   intros. assert (jj::GH = ([] ++ jj :: GH)). simpl. reflexivity. rewrite H0. *)
-(*   assert (splice (length GH) T1 = T1). apply valtp_closed in H. eapply closed_splice_idem. eassumption. omega. *)
-(*   rewrite <- H2.  *)
-(*   eapply valtp_splice_aux with (GH0 := GH). eauto. simpl. apply valtp_closed in H. eapply closed_upgrade_free. eassumption. omega. *)
-(*   simpl. apply vv in H. assumption. *)
-(* Qed. *)
+(* used in valtp_widen *)
+Lemma valtp_extendH: forall vf k H1 GH T1 vl,
+  vtp H1 GH T1 k vf ->
+  vtp H1 (vl::GH) T1 k vf.
+Proof.
+  intros. assert (vl::GH = ([] ++ vl :: GH)) by reflexivity. rewrite H0.
+  assert (splice (length GH) T1 = T1). apply valtp_closed in H. eapply closed_splice_idem. eassumption. omega.
+  rewrite <- H2.
+  eapply valtp_splice_aux with (GH0 := GH). eauto. simpl. apply valtp_closed in H. eapply closed_upgrade_free. eassumption. omega.
+  simpl. assumption.
+Qed.
 
-(* Lemma valtp_shrinkH: forall vf df k H1 GH T1 jj, *)
-(*   val_type H1 (jj::GH) T1 k (df k) vf -> *)
-(*   closed 0 (length GH) (length H1) T1 ->                      *)
-(*   vtp H1 GH T1 k (df k) vf. *)
-(* Proof. *)
-(*   intros.  *)
-(*   assert (vtp H1 ([] ++ GH) T1 k (df k) vf <->  *)
-(*   vtp H1 ([] ++ jj :: GH) (splice (length GH) T1) k (df k) vf). *)
-(*   eapply valtp_splice_aux. eauto. simpl. assumption.  *)
-(*   apply H2. simpl. assert (splice (length GH) T1 = T1). *)
-(*   eapply closed_splice_idem. eassumption. omega. apply vv in H. *)
-(*   rewrite H3. assumption.  *)
-(* Qed. *)
-
-
+Lemma valtp_shrinkH: forall vf k H1 GH T1 jj,
+  vtp H1 (jj::GH) T1 k vf ->
+  closed 0 (length GH) (length H1) T1 ->
+  vtp H1 GH T1 k vf.
+Proof.
+  intros.
+  assert (vtp H1 ([] ++ GH) T1 k vf <->
+  vtp H1 ([] ++ jj :: GH) (splice (length GH) T1) k vf).
+  eapply valtp_splice_aux. eauto. simpl. assumption.
+  apply H2. simpl. assert (splice (length GH) T1 = T1).
+  eapply closed_splice_idem. eassumption. omega.
+  rewrite H3. assumption.
+Qed.
 
 
-(* (* used in invert_abs *) *)
-(* Lemma vtp_subst1: forall venv jj v d k T2, *)
-(*   val_type venv [jj] (open (varH 0) T2) k (d k) v -> *)
-(*   closed 0 0 (length venv) T2 -> *)
-(*   val_type venv [] T2 k (d k) v. *)
-(* Proof. *)
-(*   intros. assert (open (varH 0) T2 = T2). symmetry. unfold open.  *)
-(*   eapply closed_no_open. eapply H0. rewrite H1 in H.  *)
-(*   apply unvv. eapply valtp_shrinkH. simpl. eassumption. assumption. *)
-(* Qed. *)
 
-(* Lemma vtp_subst2_aux: forall n T venv jj v x d m GH j k, *)
-(*   tsize_flat T < n -> *)
-(*   closed j (length GH) (length venv) T -> k < j -> *)
-(*   indexr x venv = Some jj -> *)
-(*   (vtp venv (GH ++ [jj]) (open_rec k (varH 0) (splice 0 T)) m (d m) v <-> *)
-(*    vtp venv GH (open_rec k (varF x) T) m (d m) v). *)
+
+(* used in invert_abs *)
+Lemma vtp_subst1: forall venv jj v k T2,
+  vtp venv [jj] (open (varH 0) T2) k v ->
+  closed 0 0 (length venv) T2 ->
+  vtp venv [] T2 k v.
+Proof.
+  intros. assert (open (varH 0) T2 = T2). symmetry. unfold open.
+  eapply closed_no_open. eapply H0. rewrite H1 in H.
+ eapply valtp_shrinkH. simpl. eassumption. assumption.
+Qed.
+
+Lemma vtp_subst2_aux: forall n T venv jj v x m GH j k,
+  tsize_flat T < n ->
+  closed j (length GH) (length venv) T -> k < j ->
+  indexr x venv = Some jj ->
+  (vtp venv (GH ++ [jj]) (open_rec k (varH 0) (splice 0 T)) m v <->
+   vtp venv GH (open_rec k (varF x) T) m v).
+Admitted.
 (* Proof. *)
 (*   induction n; intros ? ? ? ? ? ? ? ? ? ? Sz Cz Bd Id. inversion Sz. *)
 (*   destruct T; split; intros V; apply unvv in V; rewrite val_type_unfold in V. *)
@@ -1618,115 +1711,114 @@ Definition R_env venv genv tenv :=
 (* Qed. *)
 
 
-(* Lemma vtp_subst: forall T venv jj v x d k GH, *)
-(*   closed 1 (length GH) (length venv) T ->  *)
-(*   indexr x venv = Some jj -> *)
-(*   (vtp venv (GH ++ [jj]) (open (varH 0) (splice 0 T)) k (d k) v <-> *)
-(*    vtp venv GH (open (varF x) T) k (d k) v). *)
-(* Proof. intros. eapply vtp_subst2_aux. eauto. eassumption. omega. assumption. Qed. *)
+Lemma vtp_subst: forall T venv jj v x k GH,
+  closed 1 (length GH) (length venv) T ->
+  indexr x venv = Some jj ->
+  (vtp venv (GH ++ [jj]) (open (varH 0) (splice 0 T)) k v <->
+   vtp venv GH (open (varF x) T) k v).
+Proof. intros. eapply vtp_subst2_aux. eauto. eassumption. omega. assumption. Qed.
 
 
-(* (* used in invert_dabs *) *)
-(* Lemma vtp_subst2: forall venv jj v x d k  T2, *)
-(*   closed 1 0 (length venv) T2 -> *)
-(*   val_type venv [jj] (open (varH 0) T2) k (d k) v -> *)
-(*   indexr x venv = Some jj -> *)
-(*   val_type venv [] (open (varF x) T2) k (d k) v. *)
-(* Proof. *)
-(*   intros. apply vv in H0. assert ([jj] = ([] ++ [jj])). simpl. reflexivity. *)
-(*   rewrite H2 in H0. assert (splice 0 T2 = T2). eapply closed_splice_idem. *)
-(*   eassumption. omega. rewrite <- H3 in H0. eapply vtp_subst in H0. apply unvv. eassumption. *)
-(*   simpl. assumption. assumption. *)
-(* Qed. *)
+(* used in invert_dabs *)
+Lemma vtp_subst2: forall venv jj v x k  T2,
+  closed 1 0 (length venv) T2 ->
+  vtp venv [jj] (open (varH 0) T2) k v ->
+  indexr x venv = Some jj ->
+  vtp venv [] (open (varF x) T2) k v.
+Proof.
+  intros. assert ([jj] = ([] ++ [jj])). reflexivity.
+  rewrite H2 in H0. assert (splice 0 T2 = T2). eapply closed_splice_idem.
+  eassumption. omega. rewrite <- H3 in H0. eapply vtp_subst in H0. eassumption.
+  simpl. assumption. assumption.
+Qed.
 
-(* (* used in valtp_bounds *) *)
-(* Lemma vtp_subst2_general: forall venv jj v x T2 d k, *)
-(*   closed 1 0 (length venv) T2 -> *)
-(*   indexr x venv = Some jj -> *)
-(*   ( vtp venv [jj] (open (varH 0) T2) k (d k) v <-> *)
-(*     vtp venv [] (open (varF x) T2) k (d k) v). *)
-(* Proof. *)
-(*   intros. split.  *)
-(*   Case "->". intros. assert ([jj] = ([] ++ [jj])). simpl. reflexivity. *)
-(*   rewrite H2 in H1. assert (splice 0 T2 = T2). eapply closed_splice_idem. *)
-(*   eassumption. omega. rewrite <- H3 in H1. eapply vtp_subst in H1. eassumption. *)
-(*   simpl. assumption. assumption. *)
-(*   Case "<-". intros.  assert ([jj] = ([] ++ [jj])). simpl. reflexivity. *)
-(*   assert (splice 0 T2 = T2). eapply closed_splice_idem. eassumption. omega. *)
-(*   eapply vtp_subst in H1; try eassumption. rewrite <- H2 in H1. rewrite H3 in H1. *)
-(*   assumption. *)
-(* Qed. *)
+(* used in valtp_bounds *)
+Lemma vtp_subst2_general: forall venv jj v x T2 k,
+  closed 1 0 (length venv) T2 ->
+  indexr x venv = Some jj ->
+  ( vtp venv [jj] (open (varH 0) T2) k v <->
+    vtp venv [] (open (varF x) T2) k v).
+Proof.
+  intros. split.
+  Case "->". intros. assert ([jj] = ([] ++ [jj])). simpl. reflexivity.
+  rewrite H2 in H1. assert (splice 0 T2 = T2). eapply closed_splice_idem.
+  eassumption. omega. rewrite <- H3 in H1. eapply vtp_subst in H1. eassumption.
+  simpl. assumption. assumption.
+  Case "<-". intros.  assert ([jj] = ([] ++ [jj])). simpl. reflexivity.
+  assert (splice 0 T2 = T2). eapply closed_splice_idem. eassumption. omega.
+  eapply vtp_subst in H1; try eassumption. rewrite <- H2 in H1. rewrite H3 in H1.
+  assumption.
+Qed.
 
 
-(* (* used in vabs case of main theorem *) *)
-(* Lemma vtp_subst3: forall venv jj v T2 d k, *)
-(*   closed 1 0 (length venv) T2 -> *)
-(*   val_type (jj::venv) [] (open (varF (length venv)) T2) k (d k) v -> *)
-(*   val_type venv [jj] (open (varH 0) T2) k (d k) v. *)
-(* Proof. *)
-(*   intros. apply unvv. assert (splice 0 T2 = T2) as EE. eapply closed_splice_idem. eassumption. omega. *)
-(*   assert (vtp (jj::venv0) ([] ++ [jj]) (open (varH 0) (splice 0 T2)) k (d k) v). *)
-(*   assert (indexr (length venv0) (jj :: venv0) = Some jj). simpl.  *)
-(*     replace (beq_nat (length venv0) (length venv0) ) with true. reflexivity.  *)
-(*     apply beq_nat_refl.  *)
-(*   eapply vtp_subst. simpl. eapply closed_upgrade_freef. eassumption. omega. eassumption. *)
-(*   apply vv. assumption.  *)
-(*   simpl in *. rewrite EE in H1. eapply valtp_shrinkM. apply unvv. eassumption. *)
-(*   apply closed_open. simpl. eapply closed_upgrade_free. eassumption. omega. *)
-(*   constructor. simpl. omega. *)
-(* Qed. *)
+(* used in vabs case of main theorem *)
+Lemma vtp_subst3: forall venv v' v T2 k,
+  closed 1 0 (length venv) T2 ->
+  vtp (v'::venv) [] (open (varF (length venv)) T2) k v ->
+  vtp venv [v'] (open (varH 0) T2) k v.
+Proof.
+  intros. assert (splice 0 T2 = T2) as EE. eapply closed_splice_idem. eassumption. omega.
+  assert (vtp (v'::venv) ([] ++ [v']) (open (varH 0) (splice 0 T2)) k v).
+  assert (indexr (length venv) (v' :: venv) = Some v'). simpl.
+    replace (beq_nat (length venv) (length venv) ) with true. reflexivity.
+    apply beq_nat_refl.
+  eapply vtp_subst. simpl. eapply closed_upgrade_freef. eassumption. omega. eassumption.
+  assumption.
+  simpl in *. rewrite EE in H1. eapply valtp_shrinkM. eassumption.
+  apply closed_open. simpl. eapply closed_upgrade_free. eassumption. omega.
+  constructor. simpl. omega.
+Qed.
 
-(* Lemma open_preserves_size2: forall T x j, *)
-(*   tsize_flat T = tsize_flat (open_rec j (varF x) T). *)
-(* Proof. *)
-(*   intros T. induction T; intros; simpl; eauto. *)
-(*   - destruct v; simpl; destruct (beq_nat j i); eauto. *)
-(* Qed. *)
+Lemma open_preserves_size2: forall T x j,
+  tsize_flat T = tsize_flat (open_rec j (varF x) T).
+Proof.
+  intros T. induction T; intros; simpl; eauto.
+  - destruct v; simpl; destruct (beq_nat j i); eauto.
+Qed.
 
-(* Lemma valty_subst4: forall G T1 jj v d k, *)
-(*   closed 1 0 (length G) T1 -> *)
-(*   (vtp G [jj] (open (varH 0) T1) k (d k) v <-> *)
-(*    vtp (jj :: G) [] (open (varF (length G)) T1) k (d k) v).  *)
-(* Proof. *)
-(*   intros. split.  *)
-(*   Case "->". intros. assert (vtp (jj :: G) [jj] (open (varH 0) T1) k (d k) v). *)
-(*     { eapply valtp_extend_aux with (H1 := G). eauto.  *)
-(*       simpl. eapply closed_open. simpl. eapply closed_inc_mult. eassumption. omega. omega. *)
-(*       omega. constructor. omega. assumption. } *)
-(*     assert (vtp (jj :: G) [] (open (varF (length G)) T1) k (d k) v). *)
-(*     { eapply vtp_subst2_general. simpl. eapply closed_upgrade_freef. eassumption. omega. *)
-(*       simpl. replace (beq_nat (length G) (length G)) with true. reflexivity. apply beq_nat_refl.  *)
-(*       assumption. } assumption. *)
-(*   Case "<-". intros. assert (vtp (jj :: G) [jj] (open (varF (length G)) T1) k (d k) v). *)
-(*     { eapply valtp_extendH. apply unvv. assumption. } *)
-(*     assert (vtp (jj :: G) [jj] (open (varH 0) T1) k (d k) v). *)
-(*     { eapply vtp_subst2_general with (x := length G). simpl. eapply closed_upgrade_freef. eassumption. omega. *)
-(*       simpl. replace (beq_nat (length G) (length G)) with true. reflexivity. apply beq_nat_refl.  *)
-(*       eassumption. } *)
-(*     eapply valtp_shrinkM. apply unvv. eassumption. simpl. eapply closed_open. simpl. eapply closed_upgrade_free. *)
-(*     eassumption. omega. constructor. omega. *)
-(* Qed. *)
+Lemma valty_subst4: forall G T1 v' v k,
+  closed 1 0 (length G) T1 ->
+  (vtp G [v'] (open (varH 0) T1) k v <->
+   vtp (v' :: G) [] (open (varF (length G)) T1) k v).
+Proof.
+  intros. split.
+  Case "->". intros. assert (vtp (v' :: G) [v'] (open (varH 0) T1) k v).
+    { eapply valtp_extend_aux with (H1 := G). eauto.
+      simpl. eapply closed_open. simpl. eapply closed_inc_mult. eassumption. omega. omega.
+      omega. constructor. omega. assumption. }
+    assert (vtp (v' :: G) [] (open (varF (length G)) T1) k v).
+    { eapply vtp_subst2_general. simpl. eapply closed_upgrade_freef. eassumption. omega.
+      simpl. replace (beq_nat (length G) (length G)) with true. reflexivity. apply beq_nat_refl.
+      assumption. } assumption.
+  Case "<-". intros. assert (vtp (v' :: G) [v'] (open (varF (length G)) T1) k v).
+    { eapply valtp_extendH. assumption. }
+    assert (vtp (v' :: G) [v'] (open (varH 0) T1) k v).
+    { eapply vtp_subst2_general with (x := length G). simpl. eapply closed_upgrade_freef. eassumption. omega.
+      simpl. replace (beq_nat (length G) (length G)) with true. reflexivity. apply beq_nat_refl.
+      eassumption. }
+    eapply valtp_shrinkM. eassumption. simpl. eapply closed_open. simpl. eapply closed_upgrade_free.
+    eassumption. omega. constructor. omega.
+Qed.
    
 
 
 
-(* (* ### Relating Value Typing and Subtyping ### *) *)
-(* Lemma valtp_widen_aux: forall G1 GH1 T1 T2, *)
-(*   stp G1 GH1 T1 T2 -> *)
-(*   forall (H: list vseta) GH, *)
-(*     length G1 = length H -> *)
-(*     (forall x TX, indexr x G1 = Some TX -> *)
-(*                    exists vx jj, *)
-(*                      indexr x H = Some jj /\ *)
-(*                      (forall n, vtp H GH TX n (jj n) vx)) -> *)
-(*     length GH1 = length GH -> *)
-(*     (forall x TX, indexr x GH1 = Some TX -> *)
-(*                    exists vx jj, *)
-(*                      indexr x GH = Some jj /\ *)
-(*                      (forall n, vtp H GH TX n (jj n) vx)) -> *)
-(*   (forall kf (df:vseta) vf,  *)
-(*      val_type H GH T1 kf (df kf) vf -> vtp H GH T2 kf (df kf) vf). *)
-(* Proof. *)
+(* ### Relating Value Typing and Subtyping ### *)
+Lemma valtp_widen_aux: forall G1 GH1 T1 T2,
+  stp G1 GH1 T1 T2 ->
+  forall H GH,
+    length G1 = length H ->
+    (forall x TX, indexr x G1 = Some TX ->
+                   exists vx,
+                     (forall n, vtp H GH TX n vx)) ->
+    length GH1 = length GH ->
+    (forall x TX, indexr x GH1 = Some TX ->
+                   exists vx,
+                     (forall n, vtp H GH TX n vx)) ->
+  (forall kf vf,
+     vtp H GH T1 kf vf -> vtp H GH T2 kf vf).
+Proof.
+Admitted.
 (*   intros ? ? ? ? stp.  *)
 (*   induction stp; intros G GHX LG RG LGHX RGHX kf df vf V0.  *)
 
@@ -1922,52 +2014,50 @@ Definition R_env venv genv tenv :=
 (* Qed. *)
 
 
-(* Lemma valtp_widen: forall kf (df:vseta) vf GH H G1 T1 T2, *)
-(*   val_type GH [] T1 kf (df kf) vf -> *)
-(*   stp G1 [] T1 T2 -> *)
-(*   R_env H GH G1 -> *)
-(*   vtp GH [] T2 kf (df kf) vf. *)
-(* Proof. *)
-(*   intros. destruct H2 as [L1 [L2 A]]. symmetry in L2.  *)
-(*   eapply valtp_widen_aux; try eassumption; try reflexivity. *)
+Lemma valtp_widen: forall kf vf GH H G1 T1 T2,
+  vtp GH [] T1 kf  vf ->
+  stp G1 [] T1 T2 ->
+  R_env H GH G1 ->
+  vtp GH [] T2 kf  vf.
+Proof.
+  intros. destruct H2 as [L1 [L2 A]]. symmetry in L2.
+  eapply valtp_widen_aux; try eassumption; try reflexivity.
 
-(*   intros. specialize (A _ _ H2). ev. *)
-(*   eexists. eexists. split. eassumption. eassumption. *)
+  intros. specialize (A _ _ H2). ev.
+  eexists. intro. apply H4.
 
-(*   intros. inversion H2.  *)
-(* Qed. *)
+  intros. inversion H2.
+Qed.
 
 
-(* Lemma wf_env_extend: forall vx jj G1 R1 H1 T1, *)
-(*   R_env H1 R1 G1 -> *)
-(*   (forall n, val_type (jj::R1) [] T1 n (jj n) vx) -> *)
-(*   R_env (vx::H1) (jj::R1) (T1::G1). *)
-(* Proof. *)
-(*   intros. unfold R_env in *. destruct H as [L1 [L2 U]]. *)
-(*   split. simpl. rewrite L1. reflexivity. *)
-(*   split. simpl. rewrite L2. reflexivity. *)
-(*   intros. simpl in H. case_eq (beq_nat x (length G1)); intros E; rewrite E in H. *)
-(*   - inversion H. subst T1. exists jj. exists vx. *)
-(*     split. simpl. rewrite <-L1 in E. rewrite E. reflexivity. *)
-(*     split. simpl. rewrite <-L2 in E. rewrite E. reflexivity. *)
-(*     intros. eapply vv. eapply H0.  *)
-(*   - destruct (U x TX H) as [jj0 [vy0 [EV [VY IR]]]].  *)
-(*     exists jj0. exists vy0. *)
-(*     split. simpl. rewrite <-L1 in E. rewrite E. assumption. *)
-(*     split. simpl. rewrite <-L2 in E. rewrite E. assumption. *)
-(*     intros. eapply valtp_extend. eapply unvv. eapply IR.  *)
-(* Qed. *)
+Lemma wf_env_extend: forall vx vy G1 R1 H1 T1,
+  R_env H1 R1 G1 ->
+  (forall n, vtp (vy::R1) [] T1 n vx) ->
+  R_env (vx::H1) (vy::R1) (T1::G1).
+Proof.
+  intros. unfold R_env in *. destruct H as [L1 [L2 U]].
+  split. simpl. rewrite L1. reflexivity.
+  split. simpl. rewrite L2. reflexivity.
+  intros. simpl in H. case_eq (beq_nat x (length G1)); intros E; rewrite E in H.
+  - inversion H. subst T1. exists vx.
+    split. simpl. rewrite <-L1 in E. rewrite E. reflexivity.
+    intros. auto.
+  - destruct (U x TX H) as [vy0 [EV IR]].
+    exists vy0.
+    split. simpl. rewrite <-L1 in E. rewrite E. assumption.
+    intros. eapply valtp_extend. eapply IR.
+Qed.
 
-(* Lemma wf_env_extend0: forall vx jj G1 R1 H1 T1, *)
-(*   R_env H1 R1 G1 -> *)
-(*   (forall n, val_type R1 [] T1 n (jj n) vx) -> *)
-(*   R_env (vx::H1) (jj::R1) (T1::G1). *)
-(* Proof. *)
-(*   intros. *)
-(*   assert (forall n, val_type (jj::R1) [] T1 n (jj n) vx) as V0. *)
-(*   intro. eapply unvv. eapply valtp_extend. eapply H0. *)
-(*   eapply wf_env_extend; assumption. *)
-(* Qed. *)
+Lemma wf_env_extend0: forall vx vy G1 R1 H1 T1,
+  R_env H1 R1 G1 ->
+  (forall n, vtp R1 [] T1 n  vx) ->
+  R_env (vx::H1) (vy::R1) (T1::G1).
+Proof.
+  intros.
+  assert (forall n, vtp (vy::R1) [] T1 n vx) as V0.
+  intro. eapply valtp_extend. eapply H0.
+  eapply wf_env_extend; assumption.
+Qed.
 
 
 
@@ -1978,24 +2068,24 @@ Definition R_env venv genv tenv :=
 
 (* Lemma invert_var : forall x tenv T, *)
 (*   has_type tenv (tvar x) T -> forall venv renv, R_env venv renv tenv -> *)
-(*   exists (d: vseta) v, tevaln venv (tvar x) v /\ indexr x venv = Some v /\ indexr x renv = Some d /\ forall k, val_type renv [] T k (d k) v. *)
+(*   exists  v, tevaln venv (tvar x) v /\ indexr x venv = Some v /\ forall k, val_type venv [] T k v. *)
 (* Proof. *)
 (*   intros ? ? ? W. remember (tvar x) as e. *)
 (*   induction W; intros ? ? WFE; inversion Heqe; try subst x0. *)
 
-(*   - Case "Var".  *)
-(*     destruct (indexr_safe_ex venv0 renv env T1 x) as [d [v [I [D V]]]]. eauto. eauto.  *)
+(*   - Case "Var". *)
+(*     destruct (indexr_safe_ex venv0 renv env T1 x) as [d [v [I [D V]]]]. eauto. eauto. *)
     
 (*     exists d. exists v. split. exists 0. intros. destruct n. omega. simpl. rewrite I. eauto. split. apply I. split. apply D. eapply V. *)
 
 (*   - Case "VarPack". *)
 (*     unfold R_env in WFE. ev. destruct (H4 _ _ H) as [d [v [I ?]]]. ev. *)
 (*     exists d. exists v. split. exists 0. intros. destruct n. omega. simpl. rewrite I. reflexivity. *)
-(*     intros.  *)
+(*     intros. *)
 (*     assert (forall n, val_type renv [d] (open (varH 0) T1) n (d n) v). { *)
 (*       intros. eapply unvv. eapply vtp_subst2_general. rewrite H3. assumption. eassumption. eapply H6. } *)
-(*     split. assumption. split. assumption. intros. rewrite val_type_unfold. rewrite H3.  *)
-(*     destruct v; split; try assumption; exists d; (split; [reflexivity| assumption]).  *)
+(*     split. assumption. split. assumption. intros. rewrite val_type_unfold. rewrite H3. *)
+(*     destruct v; split; try assumption; exists d; (split; [reflexivity| assumption]). *)
 
 (*   - Case "And". *)
 (*     destruct (IHW1 eq_refl venv0 renv WFE) as [d1 [v1 [E1 [I1 [D1 HVF]]]]]. *)
@@ -2007,9 +2097,9 @@ Definition R_env venv genv tenv :=
 (*     intros. rewrite val_type_unfold. destruct v1; (split; [apply HVF|apply HVX]). *)
 
 (*   - Case "Sub". *)
-(*     specialize (IHW Heqe venv0 renv WFE). ev. exists x0. exists x1. split. subst e. eassumption. split. assumption. split. assumption.  *)
-(*     intros. eapply unvv. eapply valtp_widen. eapply H4. eapply H. eapply WFE.  *)
-(* Qed.  *)
+(*     specialize (IHW Heqe venv0 renv WFE). ev. exists x0. exists x1. split. subst e. eassumption. split. assumption. split. assumption. *)
+(*     intros. eapply unvv. eapply valtp_widen. eapply H4. eapply H. eapply WFE. *)
+(* Qed. *)
 
 
 (* (* main theorem *) *)
@@ -2017,38 +2107,38 @@ Definition R_env venv genv tenv :=
 (*   has_type tenv e T -> forall venv renv, R_env venv renv tenv -> *)
 (*   exists (d: vseta) v, tevaln venv e v /\ forall k, val_type renv [] T k (d k) v. *)
 (* Proof. *)
-(*   intros ? ? ? W.  *)
+(*   intros ? ? ? W. *)
 (*   induction W; intros ? ? WFE. *)
 
 (*   - Case "Var". *)
 (*     destruct (invert_var x env T1 (t_var x env T1 H H0) venv0 renv WFE) as [d [v [E [I [D V]]]]]. *)
 (*     exists d. exists v. split. apply E. apply V. *)
-(*   - Case "VarPack".  *)
+(*   - Case "VarPack". *)
 (*     destruct (invert_var x G1 (TBind T1) (t_var_pack _ x T1 T1' H H0 H1) venv0 renv WFE) as [d [v [E [I [D V]]]]]. *)
-(*     exists d. exists v. split. apply E. apply V.  *)
+(*     exists d. exists v. split. apply E. apply V. *)
 
 
-(*   - Case "unpack".  *)
-(*     rewrite <-(wf_length2 _ _ _ WFE) in H.  *)
+(*   - Case "unpack". *)
+(*     rewrite <-(wf_length2 _ _ _ WFE) in H. *)
 (*     destruct (IHW1 venv0 renv WFE) as [dx [vx [IW1 HVX]]]. *)
 (*     specialize (HVX 0). *)
 (*     rewrite val_type_unfold in HVX. *)
 (*     assert (exists jj : vseta, *)
 (*               (forall n : nat, *)
 (*                  val_type renv [jj] (open (varH 0) T1) n (jj n) vx)) as E. *)
-(*     destruct vx; ev; exists x0; assumption.  *)
-(*     destruct E as [jj VXH].  *)
+(*     destruct vx; ev; exists x0; assumption. *)
+(*     destruct E as [jj VXH]. *)
 (*     assert (forall n, val_type (jj::renv) [] (open (varF (length renv)) T1) n (jj n) vx) as VXF. { *)
 (*       assert (closed 1 0 (S (length renv)) T1). { destruct vx; ev; eapply closed_upgrade_freef; try eassumption; auto. } *)
 (*       intros. eapply vtp_subst2. assumption. eapply unvv. eapply valtp_extend. eapply VXH. *)
-(*       eapply indexr_hit2. reflexivity. reflexivity. }  *)
+(*       eapply indexr_hit2. reflexivity. reflexivity. } *)
     
 (*     assert (R_env (vx::venv0) (jj::renv) (T1'::env)) as WFE1. *)
 (*     eapply wf_env_extend. assumption. rewrite H. assumption. *)
 
 (*     specialize (IHW2 _ _ WFE1). *)
 (*     destruct IHW2 as [dy [vy [IW2 HVY]]]. *)
-(*     clear HVX. clear VXF.  *)
+(*     clear HVX. clear VXF. *)
 
 (*     exists dy. exists vy. split. { *)
 (*       destruct IW1 as [nx IWX]. *)
@@ -2057,26 +2147,26 @@ Definition R_env venv genv tenv :=
 (*       rewrite IWX. rewrite IWY. eauto. *)
 (*       omega. omega. *)
 (*     } *)
-(*     intros. eapply unvv. eapply valtp_shrink.  *)
+(*     intros. eapply unvv. eapply valtp_shrink. *)
 (*     eapply HVY. rewrite (wf_length2 _ _ _ WFE). assumption. *)
 
-(*   - Case "And".  *)
+(*   - Case "And". *)
 (*     destruct (invert_var x env (TAnd T1 T2) (t_and env x T1 T2 W1 W2) venv0 renv WFE) as [d [v [E [I [D V]]]]]. *)
-(*     exists d. exists v. split. apply E. apply V.  *)
+(*     exists d. exists v. split. apply E. apply V. *)
 
 (*   - Case "Typ". *)
 
-(*     specialize valtp_to_vseta. intros S. specialize (S renv [] T1). ev.  *)
+(*     specialize valtp_to_vseta. intros S. specialize (S renv [] T1). ev. *)
     
 (*     exists x. eexists. split. exists 1. intros. destruct n. inversion H1. simpl. reflexivity. *)
 (*     rewrite <-(wf_length2 venv0 renv) in H. *)
 (*     intros. rewrite val_type_unfold. simpl. repeat split; try eapply H. *)
-(*     destruct k. trivial. intros. destruct (H0 k (dy k) vy). split; assumption.  *)
+(*     destruct k. trivial. intros. destruct (H0 k (dy k) vy). split; assumption. *)
 (*     eapply WFE. *)
 
     
 (*   - Case "App". *)
-(*     rewrite <-(wf_length2 _ _ _ WFE) in H.  *)
+(*     rewrite <-(wf_length2 _ _ _ WFE) in H. *)
 (*     destruct (IHW1 venv0 renv WFE) as [df [vf [IW1 HVF]]]. *)
 (*     destruct (IHW2 venv0 renv WFE) as [dx [vx [IW2 HVX]]]. *)
 
@@ -2099,7 +2189,7 @@ Definition R_env venv genv tenv :=
 (*     intros. eapply vtp_subst1. eapply HVY. eapply H. *)
 
 (*   - Case "DApp". *)
-(*     rewrite <-(wf_length2 _ _ _ WFE) in H0.  *)
+(*     rewrite <-(wf_length2 _ _ _ WFE) in H0. *)
 (*     destruct (IHW1 venv0 renv WFE) as [df [vf [IW1 HVF]]]. *)
 (*     destruct (invert_var x env T1 W2 venv0 renv WFE) as [dx [vx [IW2 [I [D HVX]]]]]. *)
 
@@ -2135,13 +2225,13 @@ Definition R_env venv genv tenv :=
 (*     assert (R_env (vx::venv0) (jj::renv) (T1::env)) as WFE1. { *)
 (*       eapply wf_env_extend0. eapply WFE. eapply H0. } *)
 (*     specialize (IHW (vx::venv0) (jj::renv) WFE1). *)
-(*     destruct IHW as [d [v [EV VT]]]. rewrite <-(wf_length2 _ _ _ WFE) in VT.  *)
-(*     exists d. exists v. split. eapply EV.  *)
-(*     intros. eapply vtp_subst3. assumption. eapply VT.  *)
+(*     destruct IHW as [d [v [EV VT]]]. rewrite <-(wf_length2 _ _ _ WFE) in VT. *)
+(*     exists d. exists v. split. eapply EV. *)
+(*     intros. eapply vtp_subst3. assumption. eapply VT. *)
 
 (*   - Case "Sub". *)
 (*     specialize (IHW venv0 renv WFE). ev. exists x. exists x0. split. eassumption. *)
-(*     intros. eapply unvv. eapply valtp_widen. eapply H1. eapply H. eapply WFE.  *)
+(*     intros. eapply unvv. eapply valtp_widen. eapply H1. eapply H. eapply WFE. *)
 
 (* Grab Existential Variables. *)
 
